proof/crypto_scalarmult/curve25519/amd64/cryptoline_extraction/CommonCryptoline.ec
@@ -1,15 +1,24 @@
 require import AllCore Int IntDiv CoreMap List Distr. (* useful to include Int import *)
 
-from Jasmin require import JModel_x86.
+from Jasmin require import JModel_x86 Jcheck.
 
 import SLH64.
 
-require import Jcheck  Zp_limbs Zp_25519.
+require import Zp_limbs Zp_25519.
 import Zp_25519 Zp Zp_limbs EClib.
 
 require import WArray32.
 
 require import Array4.
+
+
+abbrev u64i x = W64.to_uint x.
+abbrev pow = Ring.IntID.exp.
+abbrev single: int -> int = idfun.
+abbrev quad (a b c d: W64.t) =  [a; b; c; d].
+abbrev limbs_4u64 (r: W64.t list) = pack4 r.  
+abbrev eqmod (a b c: int) = (a - b) %% c = 0.
+
 
 lemma limbs_are_same (f : Rep4) :
     valRep4 f = (foldr (fun x => (fun (acc: int) => (x + acc))) 0
@@ -27,7 +36,6 @@ proof.
     rewrite inzpRep4E; congr. apply limbs_are_same. 
 qed.
 
-
 lemma mul4_a24_equiv_contract (xa h: Rep4) :
       inzpRep4 h = inzp (valRep4 xa * 121665) <=>       
        (eqmod
@@ -37,30 +45,35 @@ lemma mul4_a24_equiv_contract (xa h: Rep4) :
       (map (fun ii => ((pow 2 (64 * ii)) * (u64i xa.[ii]))) (iota_ 0 4))) *
      121665) (single ((pow 2 255) - 19))).
 proof.      
-      rewrite -!limbs_are_same.
-      rewrite !inzpRep4E !/inzp. smt(@Zp_25519).      
+    do split.          
+    rewrite -!limbs_are_same.             
+    rewrite !inzpRep4E. move => H. rewrite /idfun -pE -!inzpK !inzpD inzpN !H -!inzpD //= !inzpK => />.
+    smt(@Zp_25519 @IntDiv).
+    rewrite -!limbs_are_same.             
+    rewrite !inzpRep4E. rewrite /idfun -pE -!inzpK !inzpD inzpN -!inzpD //= !inzpK => />.
+    smt(@Zp_25519 @IntDiv).       
 qed.
 
 
-lemma add4_equiv_contract (f g h: Rep4) :
-      inzpRep4 h = inzpRep4 f + inzpRep4 g <=>       
+lemma add4_equiv_contract (_f _g h: Rep4) :
+      inzpRep4 h = inzpRep4 _f + inzpRep4 _g <=>       
       (eqmod
       (foldr (fun x => (fun (acc: int) => (x + acc))) 0
       (map (fun ii => ((pow 2 (64 * ii)) * (u64i h.[ii]))) (iota_ 0 4)))
       ((foldr (fun x => (fun (acc: int) => (x + acc))) 0
-       (map (fun ii => ((pow 2 (64 * ii)) * (u64i f.[ii]))) (iota_ 0 4))) +
+       (map (fun ii => ((pow 2 (64 * ii)) * (u64i _f.[ii]))) (iota_ 0 4))) +
       (foldr (fun x => (fun (acc: int) => (x + acc))) 0
-      (map (fun ii => ((pow 2 (64 * ii)) * (u64i g.[ii]))) (iota_ 0 4))))
+      (map (fun ii => ((pow 2 (64 * ii)) * (u64i _g.[ii]))) (iota_ 0 4))))
       (single ((pow 2 255) - 19))).
 proof.
       split.
-      rewrite -!limbs_are_same.
-      rewrite inzpRep4E /inzp. smt(@Zp_25519).
-      rewrite -!limbs_are_same.
-      rewrite inzpRep4E /inzp. smt(@Zp_25519).
+      rewrite -!limbs_are_same.             
+      rewrite !inzpRep4E. move => H. rewrite /idfun -pE -!inzpK !inzpD inzpN !H -!inzpD //= !inzpK => />.
+      smt(@Zp_25519 @IntDiv).
+      rewrite -!limbs_are_same.             
+      rewrite !inzpRep4E. rewrite /idfun -pE -!inzpK !inzpD inzpN -!inzpD //= !inzpK => />.
+      smt(@Zp_25519 @IntDiv).      
 qed.
-
-    
 
 lemma mul4_equiv_contract (xa ya h: Rep4) :
       inzpRep4 h = inzp (valRep4 xa * valRep4 ya) <=>       
@@ -73,8 +86,13 @@ lemma mul4_equiv_contract (xa ya h: Rep4) :
      (map (fun ii => ((pow 2 (64 * ii)) * (u64i ya.[ii]))) (iota_ 0 4))))
      (single ((pow 2 255) - 19))).
 proof.      
-      rewrite -!limbs_are_same.
-      rewrite !inzpRep4E !/inzp. smt(@Zp_25519).      
+    do split.          
+    rewrite -!limbs_are_same.             
+    rewrite !inzpRep4E. move => H. rewrite /idfun -pE -!inzpK !inzpD inzpN !H -!inzpD //= !inzpK => />.
+    smt(@Zp_25519 @IntDiv).
+    rewrite -!limbs_are_same.             
+    rewrite !inzpRep4E. rewrite /idfun -pE -!inzpK !inzpD inzpN -!inzpD //= !inzpK => />.
+    smt(@Zp_25519 @IntDiv).          
 qed.
 
 
@@ -89,8 +107,13 @@ lemma sqr4_equiv_contract (xa h: Rep4) :
      (map (fun ii => ((pow 2 (64 * ii)) * (u64i xa.[ii]))) (iota_ 0 4))))
      (single ((pow 2 255) - 19))).
 proof.      
-      rewrite -!limbs_are_same.
-      rewrite !inzpRep4E !/inzp. smt(@Zp_25519).      
+    do split.          
+    rewrite -!limbs_are_same.             
+    rewrite !inzpRep4E. move => H. rewrite /idfun -pE -!inzpK !inzpD inzpN !H -!inzpD //= !inzpK => />.
+    smt(@Zp_25519 @IntDiv).
+    rewrite -!limbs_are_same.             
+    rewrite !inzpRep4E. rewrite /idfun -pE -!inzpK !inzpD inzpN -!inzpD //= !inzpK => />.
+    smt(@Zp_25519 @IntDiv).      
 qed.
 
 
@@ -105,9 +128,34 @@ lemma sub4_equiv_contract (f g h: Rep4) :
       (map (fun ii => ((pow 2 (64 * ii)) * (u64i g.[ii]))) (iota_ 0 4))))
       (single ((pow 2 255) - 19))).
 proof.
-      split.
-      rewrite -!limbs_are_same.
-      rewrite inzpRep4E /inzp. smt(@Zp_25519).
-      rewrite -!limbs_are_same.
-      rewrite inzpRep4E /inzp. smt(@Zp_25519).
+    do split.          
+    rewrite -!limbs_are_same.             
+    rewrite !inzpRep4E. move => H. rewrite /idfun -pE -!inzpK !inzpD inzpN !H -!inzpD //= !inzpK => />.
+    smt(@Zp_25519 @IntDiv).
+    rewrite -!limbs_are_same.             
+    rewrite !inzpRep4E. rewrite /idfun -pE -!inzpK !inzpD inzpN -!inzpD //= !inzpK => />.
+    smt(@Zp_25519 @IntDiv).
+qed.
+
+lemma tobytes_equiv_contract (h _f: Rep4) :
+      pack4 (to_list _f) = (W256.of_int (asint (inzpRep4 h))) <=>    
+      (eqmod
+      (foldr (fun x => (fun (acc:int) => (x + acc))) 0
+      (map (fun ii => ((pow 2 (64 * ii)) * (u64i h.[ii]))) (iota_ 0 4)))
+      (foldr (fun x => (fun (acc:int) => (x + acc))) 0
+      (map (fun ii => ((pow 2 (64 * ii)) * (u64i _f.[ii]))) (iota_ 0 4)))
+      (single ((pow 2 255) - 19))).
+proof.    
+    auto => />. do split. move => H. 
+    rewrite -!limbs_are_same /idfun.    
+    have E: to_uint (limbs_4u64 (quad _f.[0] _f.[1] _f.[2] _f.[3])) = valRep4 _f.
+      + by rewrite valRep4ToPack /to_list /mkseq -iotaredE => />.
+    have E0: to_uint (limbs_4u64 (quad h.[0] h.[1] h.[2] h.[3])) = valRep4 h.
+      + by rewrite valRep4ToPack /to_list /mkseq -iotaredE => />.                            
+    have E1: limbs_4u64 (quad _f.[0] _f.[1] _f.[2] _f.[3]) = (of_int (asint (inzpRep4 h)))%W256.
+      + move: H. by rewrite/to_list /mkseq -iotaredE => />.
+    have E2: W256.to_uint (limbs_4u64 (quad _f.[0] _f.[1] _f.[2] _f.[3])) = (asint (inzpRep4 h)).
+      rewrite E1. by rewrite to_uint_small; 1:smt(ge0_asint gtp_asint pVal).
+    rewrite -E E2 inzpRep4E inzpK. smt(@IntDiv @Zp_25519 @Zp_limbs @W256).
+    admit.
 qed.
