proof/crypto_scalarmult/curve25519/amd64/cryptoline_extraction/Mul4MulxExtracted.ec
@@ -4,19 +4,17 @@ from Jasmin require import JModel_x86.
 
 import SLH64.
 
-require import Jcheck.
+from Jasmin require import Jcheck.
 
 require import Array4.
 
 require import WArray32.
 
-
-require import Jcheck Zp_limbs Zp_25519 CommonCryptoline.
+require import Zp_limbs Zp_25519 CommonCryptoline.
 import Zp_25519 Zp Zp_limbs EClib.
 
-
 module M = {
-  var tmp__check : to_check
+  var tmp__trace : trace
   var tmp__data___reduce4 : (W64.t Array4.t)
   var tmp____reduce4 : W64.t Array4.t
   var tmp__data___mul4_c0 : (W64.t Array4.t * W64.t Array4.t * bool * bool)
@@ -42,7 +40,7 @@ module M = {
   var tmp__data___mul4_rsr : (W64.t Array4.t)
   var tmp____mul4_rsr : W64.t Array4.t
   proc __reduce4 (x:W64.t Array4.t, r:W64.t Array4.t, _38:W64.t, z:W64.t,
-                  cf:bool, of_0:bool) : ((W64.t Array4.t) * to_check) = {
+                  cf:bool, of_0:bool) : ((W64.t Array4.t) * trace) = {
     var aux:bool;
     var aux_1:W64.t;
     var aux_0:W64.t;
@@ -56,14 +54,20 @@ module M = {
     var  _2:bool;
     var  _3:bool;
     var  _4:bool;
-    var assume___reduce4:bool;
-    var assert___reduce4:bool;
-    var assume_proof___reduce4:bool;
-    var assert_proof___reduce4:bool;
-    assume___reduce4 <- true;
-    assert___reduce4 <- true;
-    assume_proof___reduce4 <- true;
-    assert_proof___reduce4 <- assert___reduce4;
+    var old_of:bool;
+    var old_cf:bool;
+    var old_z:W64.t;
+    var old__38:W64.t;
+    var old_r:W64.t Array4.t;
+    var old_x:W64.t Array4.t;
+    var trace___reduce4:trace;
+    old_x <- x;
+    old_r <- r;
+    old__38 <- _38;
+    old_z <- z;
+    old_cf <- cf;
+    old_of <- of_0;
+    trace___reduce4 <- [];
     h <- witness;
     h0 <- witness;
     z <- (W64.of_int 0);
@@ -104,22 +108,10 @@ module M = {
     of_0 <- aux;
     h0.[0] <- aux_1;
     ( _0,  _1,  _2,  _3,  _4, lo) <- (IMULri_64 h0.[0] (W64.of_int 38));
-    assert_proof___reduce4 <-
-    (assert_proof___reduce4 /\
-    ((assert___reduce4 /\ assume___reduce4) => (! cf)));
-    assert___reduce4 <- (assert___reduce4 /\ (! cf));
-    assume_proof___reduce4 <-
-    (assume_proof___reduce4 /\
-    ((assert___reduce4 /\ assume___reduce4) => ((b2i cf) = 0)));
-    assume___reduce4 <- (assume___reduce4 /\ ((b2i cf) = 0));
-    assert_proof___reduce4 <-
-    (assert_proof___reduce4 /\
-    ((assert___reduce4 /\ assume___reduce4) => (! of_0)));
-    assert___reduce4 <- (assert___reduce4 /\ (! of_0));
-    assume_proof___reduce4 <-
-    (assume_proof___reduce4 /\
-    ((assert___reduce4 /\ assume___reduce4) => ((b2i of_0) = 0)));
-    assume___reduce4 <- (assume___reduce4 /\ ((b2i of_0) = 0));
+    trace___reduce4 <- (trace___reduce4 ++ [(Assert, (! cf))]);
+    trace___reduce4 <- (trace___reduce4 ++ [(Assume, ((b2i cf) = 0))]);
+    trace___reduce4 <- (trace___reduce4 ++ [(Assert, (! of_0))]);
+    trace___reduce4 <- (trace___reduce4 ++ [(Assume, ((b2i of_0) = 0))]);
     (aux, aux_1) <- (adc_64 h.[0] lo false);
     cf <- aux;
     h.[0] <- aux_1;
@@ -134,57 +126,54 @@ module M = {
     h.[3] <- aux_1;
     carryo <- cf;
     (cf, z) <- (sbb_64 z z cf);
-    assert_proof___reduce4 <-
-    (assert_proof___reduce4 /\
-    ((assert___reduce4 /\ assume___reduce4) => (cf = carryo)));
-    assert___reduce4 <- (assert___reduce4 /\ (cf = carryo));
-    assume_proof___reduce4 <-
-    (assume_proof___reduce4 /\
-    ((assert___reduce4 /\ assume___reduce4) => ((b2i cf) = (b2i carryo))));
-    assume___reduce4 <- (assume___reduce4 /\ ((b2i cf) = (b2i carryo)));
+    trace___reduce4 <- (trace___reduce4 ++ [(Assert, (cf = carryo))]);
+    trace___reduce4 <-
+    (trace___reduce4 ++ [(Assume, ((b2i cf) = (b2i carryo)))]);
     z <- (z `&` (W64.of_int 38));
-    assert_proof___reduce4 <-
-    (assert_proof___reduce4 /\
-    ((assert___reduce4 /\ assume___reduce4) =>
-    (((! cf) /\ (z = (W64.of_int 0))) \/ (cf /\ (z = (W64.of_int 38))))));
-    assert___reduce4 <-
-    (assert___reduce4 /\
-    (((! cf) /\ (z = (W64.of_int 0))) \/ (cf /\ (z = (W64.of_int 38)))));
-    assume_proof___reduce4 <-
-    (assume_proof___reduce4 /\
-    ((assert___reduce4 /\ assume___reduce4) => ((u64i z) = ((b2i cf) * 38))));
-    assume___reduce4 <- (assume___reduce4 /\ ((u64i z) = ((b2i cf) * 38)));
+    trace___reduce4 <-
+    (trace___reduce4 ++
+    [(Assert,
+     (((! cf) /\ (z = (W64.of_int 0))) \/ (cf /\ (z = (W64.of_int 38)))))]);
+    trace___reduce4 <-
+    (trace___reduce4 ++ [(Assume, ((u64i z) = ((b2i cf) * 38)))]);
     (aux, aux_1) <- (adc_64 h.[0] z false);
     cf <- aux;
     h.[0] <- aux_1;
-    assert_proof___reduce4 <-
-    (assert_proof___reduce4 /\
-    ((assert___reduce4 /\ assume___reduce4) => (! cf)));
-    assert___reduce4 <- (assert___reduce4 /\ (! cf));
-    assume_proof___reduce4 <-
-    (assume_proof___reduce4 /\
-    ((assert___reduce4 /\ assume___reduce4) => ((b2i cf) = 0)));
-    assume___reduce4 <- (assume___reduce4 /\ ((b2i cf) = 0));
-    return (h,
-           (assume___reduce4, assert___reduce4, assume_proof___reduce4,
-           assert_proof___reduce4));
+    trace___reduce4 <- (trace___reduce4 ++ [(Assert, (! cf))]);
+    trace___reduce4 <- (trace___reduce4 ++ [(Assume, ((b2i cf) = 0))]);
+    trace___reduce4 <-
+    (trace___reduce4 ++
+    [(Assert,
+     (eqmod
+     (foldr (fun x => (fun (acc:int) => (x + acc))) 0
+     (map (fun ii => ((pow 2 (64 * ii)) * (u64i h.[ii]))) (iota_ 0 4)))
+     ((foldr (fun x => (fun (acc:int) => (x + acc))) 0
+      (map (fun ii => ((pow 2 (64 * ii)) * (u64i old_x.[ii]))) (iota_ 0 4))) +
+     (foldr (fun x => (fun (acc:int) => (x + acc))) 0
+     (map (fun ii => ((pow 2 (64 * (ii + 4))) * (u64i old_r.[ii])))
+     (iota_ 0 4)))) (single ((pow 2 255) - 19))))]);
+    return (h, trace___reduce4);
   }
   proc __mul4_c0 (f0:W64.t, g:W64.t Array4.t, z:W64.t, cf:bool, of_0:bool) : 
-  ((W64.t Array4.t * W64.t Array4.t * bool * bool) * to_check) = {
+  ((W64.t Array4.t * W64.t Array4.t * bool * bool) * trace) = {
     var aux_1:bool;
     var aux_0:W64.t;
     var aux:W64.t;
     var h:W64.t Array4.t;
     var r:W64.t Array4.t;
     var lo:W64.t;
-    var assume___mul4_c0:bool;
-    var assert___mul4_c0:bool;
-    var assume_proof___mul4_c0:bool;
-    var assert_proof___mul4_c0:bool;
-    assume___mul4_c0 <- true;
-    assert___mul4_c0 <- true;
-    assume_proof___mul4_c0 <- true;
-    assert_proof___mul4_c0 <- assert___mul4_c0;
+    var old_of:bool;
+    var old_cf:bool;
+    var old_z:W64.t;
+    var old_g:W64.t Array4.t;
+    var old_f0:W64.t;
+    var trace___mul4_c0:trace;
+    old_f0 <- f0;
+    old_g <- g;
+    old_z <- z;
+    old_cf <- cf;
+    old_of <- of_0;
+    trace___mul4_c0 <- [];
     h <- witness;
     r <- witness;
     (aux_0, aux) <- (MULX_64 f0 g.[0]);
@@ -211,37 +200,37 @@ module M = {
     (aux_1, aux_0) <- (ADCX_64 r.[0] z cf);
     cf <- aux_1;
     r.[0] <- aux_0;
-    assert_proof___mul4_c0 <-
-    (assert_proof___mul4_c0 /\
-    ((assert___mul4_c0 /\ assume___mul4_c0) => (! cf)));
-    assert___mul4_c0 <- (assert___mul4_c0 /\ (! cf));
-    assume_proof___mul4_c0 <-
-    (assume_proof___mul4_c0 /\
-    ((assert___mul4_c0 /\ assume___mul4_c0) => ((b2i cf) = 0)));
-    assume___mul4_c0 <- (assume___mul4_c0 /\ ((b2i cf) = 0));
-    return ((h, r, cf, of_0),
-           (assume___mul4_c0, assert___mul4_c0, assume_proof___mul4_c0,
-           assert_proof___mul4_c0));
+    trace___mul4_c0 <- (trace___mul4_c0 ++ [(Assert, (! cf))]);
+    trace___mul4_c0 <- (trace___mul4_c0 ++ [(Assume, ((b2i cf) = 0))]);
+    return ((h, r, cf, of_0), trace___mul4_c0);
   }
   proc __mul4_c1 (h:W64.t Array4.t, r:W64.t Array4.t, f:W64.t,
                   g:W64.t Array4.t, z:W64.t, cf:bool, of_0:bool) : ((W64.t Array4.t *
                                                                     W64.t Array4.t *
                                                                     bool *
                                                                     bool) *
-                                                                   to_check) = {
+                                                                   trace) = {
     var aux:bool;
     var aux_1:W64.t;
     var aux_0:W64.t;
     var hi:W64.t;
     var lo:W64.t;
-    var assume___mul4_c1:bool;
-    var assert___mul4_c1:bool;
-    var assume_proof___mul4_c1:bool;
-    var assert_proof___mul4_c1:bool;
-    assume___mul4_c1 <- true;
-    assert___mul4_c1 <- true;
-    assume_proof___mul4_c1 <- true;
-    assert_proof___mul4_c1 <- assert___mul4_c1;
+    var old_of:bool;
+    var old_cf:bool;
+    var old_z:W64.t;
+    var old_g:W64.t Array4.t;
+    var old_f:W64.t;
+    var old_r:W64.t Array4.t;
+    var old_h:W64.t Array4.t;
+    var trace___mul4_c1:trace;
+    old_h <- h;
+    old_r <- r;
+    old_f <- f;
+    old_g <- g;
+    old_z <- z;
+    old_cf <- cf;
+    old_of <- of_0;
+    trace___mul4_c1 <- [];
     (hi, lo) <- (MULX_64 f g.[0]);
     (aux, aux_1) <- (ADOX_64 h.[1] lo of_0);
     of_0 <- aux;
@@ -275,45 +264,39 @@ module M = {
     (aux, aux_1) <- (ADOX_64 r.[1] z of_0);
     of_0 <- aux;
     r.[1] <- aux_1;
-    assert_proof___mul4_c1 <-
-    (assert_proof___mul4_c1 /\
-    ((assert___mul4_c1 /\ assume___mul4_c1) => (! cf)));
-    assert___mul4_c1 <- (assert___mul4_c1 /\ (! cf));
-    assume_proof___mul4_c1 <-
-    (assume_proof___mul4_c1 /\
-    ((assert___mul4_c1 /\ assume___mul4_c1) => ((b2i cf) = 0)));
-    assume___mul4_c1 <- (assume___mul4_c1 /\ ((b2i cf) = 0));
-    assert_proof___mul4_c1 <-
-    (assert_proof___mul4_c1 /\
-    ((assert___mul4_c1 /\ assume___mul4_c1) => (! of_0)));
-    assert___mul4_c1 <- (assert___mul4_c1 /\ (! of_0));
-    assume_proof___mul4_c1 <-
-    (assume_proof___mul4_c1 /\
-    ((assert___mul4_c1 /\ assume___mul4_c1) => ((b2i of_0) = 0)));
-    assume___mul4_c1 <- (assume___mul4_c1 /\ ((b2i of_0) = 0));
-    return ((h, r, cf, of_0),
-           (assume___mul4_c1, assert___mul4_c1, assume_proof___mul4_c1,
-           assert_proof___mul4_c1));
+    trace___mul4_c1 <- (trace___mul4_c1 ++ [(Assert, (! cf))]);
+    trace___mul4_c1 <- (trace___mul4_c1 ++ [(Assume, ((b2i cf) = 0))]);
+    trace___mul4_c1 <- (trace___mul4_c1 ++ [(Assert, (! of_0))]);
+    trace___mul4_c1 <- (trace___mul4_c1 ++ [(Assume, ((b2i of_0) = 0))]);
+    return ((h, r, cf, of_0), trace___mul4_c1);
   }
   proc __mul4_c2 (h:W64.t Array4.t, r:W64.t Array4.t, f:W64.t,
                   g:W64.t Array4.t, z:W64.t, cf:bool, of_0:bool) : ((W64.t Array4.t *
                                                                     W64.t Array4.t *
                                                                     bool *
                                                                     bool) *
-                                                                   to_check) = {
+                                                                   trace) = {
     var aux:bool;
     var aux_1:W64.t;
     var aux_0:W64.t;
     var hi:W64.t;
     var lo:W64.t;
-    var assume___mul4_c2:bool;
-    var assert___mul4_c2:bool;
-    var assume_proof___mul4_c2:bool;
-    var assert_proof___mul4_c2:bool;
-    assume___mul4_c2 <- true;
-    assert___mul4_c2 <- true;
-    assume_proof___mul4_c2 <- true;
-    assert_proof___mul4_c2 <- assert___mul4_c2;
+    var old_of:bool;
+    var old_cf:bool;
+    var old_z:W64.t;
+    var old_g:W64.t Array4.t;
+    var old_f:W64.t;
+    var old_r:W64.t Array4.t;
+    var old_h:W64.t Array4.t;
+    var trace___mul4_c2:trace;
+    old_h <- h;
+    old_r <- r;
+    old_f <- f;
+    old_g <- g;
+    old_z <- z;
+    old_cf <- cf;
+    old_of <- of_0;
+    trace___mul4_c2 <- [];
     (hi, lo) <- (MULX_64 f g.[0]);
     (aux, aux_1) <- (ADOX_64 h.[2] lo of_0);
     of_0 <- aux;
@@ -347,45 +330,39 @@ module M = {
     (aux, aux_1) <- (ADOX_64 r.[2] z of_0);
     of_0 <- aux;
     r.[2] <- aux_1;
-    assert_proof___mul4_c2 <-
-    (assert_proof___mul4_c2 /\
-    ((assert___mul4_c2 /\ assume___mul4_c2) => (! cf)));
-    assert___mul4_c2 <- (assert___mul4_c2 /\ (! cf));
-    assume_proof___mul4_c2 <-
-    (assume_proof___mul4_c2 /\
-    ((assert___mul4_c2 /\ assume___mul4_c2) => ((b2i cf) = 0)));
-    assume___mul4_c2 <- (assume___mul4_c2 /\ ((b2i cf) = 0));
-    assert_proof___mul4_c2 <-
-    (assert_proof___mul4_c2 /\
-    ((assert___mul4_c2 /\ assume___mul4_c2) => (! of_0)));
-    assert___mul4_c2 <- (assert___mul4_c2 /\ (! of_0));
-    assume_proof___mul4_c2 <-
-    (assume_proof___mul4_c2 /\
-    ((assert___mul4_c2 /\ assume___mul4_c2) => ((b2i of_0) = 0)));
-    assume___mul4_c2 <- (assume___mul4_c2 /\ ((b2i of_0) = 0));
-    return ((h, r, cf, of_0),
-           (assume___mul4_c2, assert___mul4_c2, assume_proof___mul4_c2,
-           assert_proof___mul4_c2));
+    trace___mul4_c2 <- (trace___mul4_c2 ++ [(Assert, (! cf))]);
+    trace___mul4_c2 <- (trace___mul4_c2 ++ [(Assume, ((b2i cf) = 0))]);
+    trace___mul4_c2 <- (trace___mul4_c2 ++ [(Assert, (! of_0))]);
+    trace___mul4_c2 <- (trace___mul4_c2 ++ [(Assume, ((b2i of_0) = 0))]);
+    return ((h, r, cf, of_0), trace___mul4_c2);
   }
   proc __mul4_c3 (h:W64.t Array4.t, r:W64.t Array4.t, f:W64.t,
                   g:W64.t Array4.t, z:W64.t, cf:bool, of_0:bool) : ((W64.t Array4.t *
                                                                     W64.t Array4.t *
                                                                     bool *
                                                                     bool) *
-                                                                   to_check) = {
+                                                                   trace) = {
     var aux:bool;
     var aux_1:W64.t;
     var aux_0:W64.t;
     var hi:W64.t;
     var lo:W64.t;
-    var assume___mul4_c3:bool;
-    var assert___mul4_c3:bool;
-    var assume_proof___mul4_c3:bool;
-    var assert_proof___mul4_c3:bool;
-    assume___mul4_c3 <- true;
-    assert___mul4_c3 <- true;
-    assume_proof___mul4_c3 <- true;
-    assert_proof___mul4_c3 <- assert___mul4_c3;
+    var old_of:bool;
+    var old_cf:bool;
+    var old_z:W64.t;
+    var old_g:W64.t Array4.t;
+    var old_f:W64.t;
+    var old_r:W64.t Array4.t;
+    var old_h:W64.t Array4.t;
+    var trace___mul4_c3:trace;
+    old_h <- h;
+    old_r <- r;
+    old_f <- f;
+    old_g <- g;
+    old_z <- z;
+    old_cf <- cf;
+    old_of <- of_0;
+    trace___mul4_c3 <- [];
     (hi, lo) <- (MULX_64 f g.[0]);
     (aux, aux_1) <- (ADOX_64 h.[3] lo of_0);
     of_0 <- aux;
@@ -419,440 +396,475 @@ module M = {
     (aux, aux_1) <- (ADOX_64 r.[3] z of_0);
     of_0 <- aux;
     r.[3] <- aux_1;
-    assert_proof___mul4_c3 <-
-    (assert_proof___mul4_c3 /\
-    ((assert___mul4_c3 /\ assume___mul4_c3) => (! cf)));
-    assert___mul4_c3 <- (assert___mul4_c3 /\ (! cf));
-    assume_proof___mul4_c3 <-
-    (assume_proof___mul4_c3 /\
-    ((assert___mul4_c3 /\ assume___mul4_c3) => ((b2i cf) = 0)));
-    assume___mul4_c3 <- (assume___mul4_c3 /\ ((b2i cf) = 0));
-    assert_proof___mul4_c3 <-
-    (assert_proof___mul4_c3 /\
-    ((assert___mul4_c3 /\ assume___mul4_c3) => (! of_0)));
-    assert___mul4_c3 <- (assert___mul4_c3 /\ (! of_0));
-    assume_proof___mul4_c3 <-
-    (assume_proof___mul4_c3 /\
-    ((assert___mul4_c3 /\ assume___mul4_c3) => ((b2i of_0) = 0)));
-    assume___mul4_c3 <- (assume___mul4_c3 /\ ((b2i of_0) = 0));
-    return ((h, r, cf, of_0),
-           (assume___mul4_c3, assert___mul4_c3, assume_proof___mul4_c3,
-           assert_proof___mul4_c3));
+    trace___mul4_c3 <- (trace___mul4_c3 ++ [(Assert, (! cf))]);
+    trace___mul4_c3 <- (trace___mul4_c3 ++ [(Assume, ((b2i cf) = 0))]);
+    trace___mul4_c3 <- (trace___mul4_c3 ++ [(Assert, (! of_0))]);
+    trace___mul4_c3 <- (trace___mul4_c3 ++ [(Assume, ((b2i of_0) = 0))]);
+    return ((h, r, cf, of_0), trace___mul4_c3);
   }
   proc __mul4_rsr (fs:W64.t Array4.t, g:W64.t Array4.t) : ((W64.t Array4.t) *
-                                                          to_check) = {
+                                                          trace) = {
     var h:W64.t Array4.t;
     var of_0:bool;
     var cf:bool;
     var z:W64.t;
+    var g0:W64.t Array4.t;
     var f:W64.t;
     var r:W64.t Array4.t;
     var _38:W64.t;
     var  _0:bool;
     var  _1:bool;
     var  _2:bool;
-    var assume___mul4_rsr:bool;
-    var assert___mul4_rsr:bool;
-    var assume_proof___mul4_rsr:bool;
-    var assert_proof___mul4_rsr:bool;
-    assume___mul4_rsr <- true;
-    assert___mul4_rsr <- true;
-    assume_proof___mul4_rsr <- true;
-    assert_proof___mul4_rsr <- assert___mul4_rsr;
+    var old_g:W64.t Array4.t;
+    var old_fs:W64.t Array4.t;
+    var trace___mul4_rsr:trace;
+    old_fs <- fs;
+    old_g <- g;
+    trace___mul4_rsr <- [];
+    g0 <- witness;
     h <- witness;
     r <- witness;
     (of_0, cf,  _0,  _1,  _2, z) <- (set0_64);
+    g0 <- (copy_64 g);
     f <- fs.[0];
-    (tmp__data___mul4_c0, tmp__check) <@ __mul4_c0 (f, g, z, cf, of_0);
+    (tmp__data___mul4_c0, tmp__trace) <@ __mul4_c0 (f, g0, z, cf, of_0);
     (tmp____mul4_c0, tmp____mul4_c0_0, tmp____mul4_c0_1, tmp____mul4_c0_2) <-
     tmp__data___mul4_c0;
-    (assume___mul4_rsr, assert___mul4_rsr, assume_proof___mul4_rsr,
-    assert_proof___mul4_rsr) <-
-    (upd_call
-    (assume___mul4_rsr, assert___mul4_rsr, assume_proof___mul4_rsr,
-    assert_proof___mul4_rsr) tmp__check);
+    trace___mul4_rsr <- (trace___mul4_rsr ++ tmp__trace);
     h <- tmp____mul4_c0;
     r <- tmp____mul4_c0_0;
     cf <- tmp____mul4_c0_1;
     of_0 <- tmp____mul4_c0_2;
     f <- fs.[1];
-    (tmp__data___mul4_c1, tmp__check) <@ __mul4_c1 (h, r, f, g, z, cf, of_0);
+    (tmp__data___mul4_c1, tmp__trace) <@ __mul4_c1 (h, r, f, g0, z, cf,
+    of_0);
     (tmp____mul4_c1, tmp____mul4_c1_0, tmp____mul4_c1_1, tmp____mul4_c1_2) <-
     tmp__data___mul4_c1;
-    (assume___mul4_rsr, assert___mul4_rsr, assume_proof___mul4_rsr,
-    assert_proof___mul4_rsr) <-
-    (upd_call
-    (assume___mul4_rsr, assert___mul4_rsr, assume_proof___mul4_rsr,
-    assert_proof___mul4_rsr) tmp__check);
+    trace___mul4_rsr <- (trace___mul4_rsr ++ tmp__trace);
     h <- tmp____mul4_c1;
     r <- tmp____mul4_c1_0;
     cf <- tmp____mul4_c1_1;
     of_0 <- tmp____mul4_c1_2;
     f <- fs.[2];
-    (tmp__data___mul4_c2, tmp__check) <@ __mul4_c2 (h, r, f, g, z, cf, of_0);
+    (tmp__data___mul4_c2, tmp__trace) <@ __mul4_c2 (h, r, f, g0, z, cf,
+    of_0);
     (tmp____mul4_c2, tmp____mul4_c2_0, tmp____mul4_c2_1, tmp____mul4_c2_2) <-
     tmp__data___mul4_c2;
-    (assume___mul4_rsr, assert___mul4_rsr, assume_proof___mul4_rsr,
-    assert_proof___mul4_rsr) <-
-    (upd_call
-    (assume___mul4_rsr, assert___mul4_rsr, assume_proof___mul4_rsr,
-    assert_proof___mul4_rsr) tmp__check);
+    trace___mul4_rsr <- (trace___mul4_rsr ++ tmp__trace);
     h <- tmp____mul4_c2;
     r <- tmp____mul4_c2_0;
     cf <- tmp____mul4_c2_1;
     of_0 <- tmp____mul4_c2_2;
     f <- fs.[3];
-    (tmp__data___mul4_c3, tmp__check) <@ __mul4_c3 (h, r, f, g, z, cf, of_0);
+    (tmp__data___mul4_c3, tmp__trace) <@ __mul4_c3 (h, r, f, g0, z, cf,
+    of_0);
     (tmp____mul4_c3, tmp____mul4_c3_0, tmp____mul4_c3_1, tmp____mul4_c3_2) <-
     tmp__data___mul4_c3;
-    (assume___mul4_rsr, assert___mul4_rsr, assume_proof___mul4_rsr,
-    assert_proof___mul4_rsr) <-
-    (upd_call
-    (assume___mul4_rsr, assert___mul4_rsr, assume_proof___mul4_rsr,
-    assert_proof___mul4_rsr) tmp__check);
+    trace___mul4_rsr <- (trace___mul4_rsr ++ tmp__trace);
     h <- tmp____mul4_c3;
     r <- tmp____mul4_c3_0;
     cf <- tmp____mul4_c3_1;
     of_0 <- tmp____mul4_c3_2;
     _38 <- (W64.of_int 38);
-    (tmp__data___reduce4, tmp__check) <@ __reduce4 (h, r, _38, z, cf, of_0);
+    (tmp__data___reduce4, tmp__trace) <@ __reduce4 (h, r, _38, z, cf, of_0);
     tmp____reduce4 <- tmp__data___reduce4;
-    (assume___mul4_rsr, assert___mul4_rsr, assume_proof___mul4_rsr,
-    assert_proof___mul4_rsr) <-
-    (upd_call
-    (assume___mul4_rsr, assert___mul4_rsr, assume_proof___mul4_rsr,
-    assert_proof___mul4_rsr) tmp__check);
-    assert_proof___mul4_rsr <-
-    (assert_proof___mul4_rsr /\
-    ((assert___mul4_rsr /\ assume___mul4_rsr) =>
-    (eqmod
-    (foldr (fun x => (fun (acc: int) => (x + acc))) 0
-    (map (fun ii => ((pow 2 (64 * ii)) * (u64i tmp____reduce4.[ii])))
-    (iota_ 0 4)))
-    ((foldr (fun x => (fun (acc: int) => (x + acc))) 0
-     (map (fun ii => ((pow 2 (64 * ii)) * (u64i h.[ii]))) (iota_ 0 4))) +
-    (foldr (fun x => (fun (acc: int) => (x + acc))) 0
-    (map (fun ii => ((pow 2 (64 * (ii + 4))) * (u64i r.[ii]))) (iota_ 0 4))))
-    (single ((pow 2 255) - 19)))));
-    assert___mul4_rsr <-
-    (assert___mul4_rsr /\
-    (eqmod
-    (foldr (fun x => (fun (acc: int) => (x + acc))) 0
-    (map (fun ii => ((pow 2 (64 * ii)) * (u64i tmp____reduce4.[ii])))
-    (iota_ 0 4)))
-    ((foldr (fun x => (fun (acc: int) => (x + acc))) 0
-     (map (fun ii => ((pow 2 (64 * ii)) * (u64i h.[ii]))) (iota_ 0 4))) +
-    (foldr (fun x => (fun (acc: int) => (x + acc))) 0
-    (map (fun ii => ((pow 2 (64 * (ii + 4))) * (u64i r.[ii]))) (iota_ 0 4))))
-    (single ((pow 2 255) - 19))));
+    trace___mul4_rsr <- (trace___mul4_rsr ++ tmp__trace);
+    trace___mul4_rsr <-
+    (trace___mul4_rsr ++
+    [(Assume,
+     (eqmod
+     (foldr (fun x => (fun (acc:int) => (x + acc))) 0
+     (map (fun ii => ((pow 2 (64 * ii)) * (u64i tmp____reduce4.[ii])))
+     (iota_ 0 4)))
+     ((foldr (fun x => (fun (acc:int) => (x + acc))) 0
+      (map (fun ii => ((pow 2 (64 * ii)) * (u64i h.[ii]))) (iota_ 0 4))) +
+     (foldr (fun x => (fun (acc:int) => (x + acc))) 0
+     (map (fun ii => ((pow 2 (64 * (ii + 4))) * (u64i r.[ii]))) (iota_ 0 4))))
+     (single ((pow 2 255) - 19))))]);
     h <- tmp____reduce4;
-    return (h,
-           (assume___mul4_rsr, assert___mul4_rsr, assume_proof___mul4_rsr,
-           assert_proof___mul4_rsr));
+    trace___mul4_rsr <-
+    (trace___mul4_rsr ++
+    [(Assert,
+     (eqmod
+     (foldr (fun x => (fun (acc:int) => (x + acc))) 0
+     (map (fun ii => ((pow 2 (64 * ii)) * (u64i h.[ii]))) (iota_ 0 4)))
+     ((foldr (fun x => (fun (acc:int) => (x + acc))) 0
+      (map (fun ii => ((pow 2 (64 * ii)) * (u64i old_fs.[ii]))) (iota_ 0 4))) *
+     (foldr (fun x => (fun (acc:int) => (x + acc))) 0
+     (map (fun ii => ((pow 2 (64 * ii)) * (u64i old_g.[ii]))) (iota_ 0 4))))
+     (single ((pow 2 255) - 19))))]);
+    return (h, trace___mul4_rsr);
   }
 }.
 
-(* All assume are valid. *)
+(* The post is in the trace. *)
 
-lemma __reduce4_assume  : hoare [M.__reduce4 : true ==> (assume_proof_ res)].
+lemma __reduce4_valid_post _x _r __38 _z _cf _of :
+      hoare [M.__reduce4 :
+      ((_of = of_0) /\
+      ((_cf = cf) /\ ((_z = z) /\ ((__38 = _38) /\ ((_r = r) /\ (_x = x)))))) ==>
+      ((valid (trace res)) =>
+      (eqmod
+      (foldr (fun x => (fun (acc:int) => (x + acc))) 0
+      (map (fun ii => ((pow 2 (64 * ii)) * (u64i res.`1.[ii]))) (iota_ 0 4)))
+      ((foldr (fun x => (fun (acc:int) => (x + acc))) 0
+       (map (fun ii => ((pow 2 (64 * ii)) * (u64i _x.[ii]))) (iota_ 0 4))) +
+      (foldr (fun x => (fun (acc:int) => (x + acc))) 0
+      (map (fun ii => ((pow 2 (64 * (ii + 4))) * (u64i _r.[ii]))) (iota_ 0 4)
+      ))) (single ((pow 2 255) - 19))))].
 proof.
-    proc. 
-    seq 52 : (assume_proof__ (assume___reduce4, assert___reduce4, assume_proof___reduce4, assert_proof___reduce4)). auto => />.
-    seq 23 : (assume_proof__ (assume___reduce4, assert___reduce4, assume_proof___reduce4, assert_proof___reduce4)). auto => />.    
-    move => &hr. smt(@Zp_25519 @W64 @JUtils).
-    auto => />.
+proc .
+wp -1 => /=. auto => />.
+qed .
+
+lemma __mul4_c0_valid_post _f0 _g _z _cf _of :
+      hoare [M.__mul4_c0 :
+      ((_of = of_0) /\ ((_cf = cf) /\ ((_z = z) /\ ((_g = g) /\ (_f0 = f0))))) ==>
+      ((valid (trace res)) => true)].
+proof.
+proc .
+wp -1 => /=. auto => />.
 qed.
 
-lemma __mul4_c0_assume  : hoare [M.__mul4_c0 : true ==> (assume_proof_ res)].
+lemma __mul4_c1_valid_post _h _r _f _g _z _cf _of :
+      hoare [M.__mul4_c1 :
+      ((_of = of_0) /\
+      ((_cf = cf) /\
+      ((_z = z) /\ ((_g = g) /\ ((_f = f) /\ ((_r = r) /\ (_h = h))))))) ==>
+      ((valid (trace res)) => true)].
 proof.
-    proc. 
-    seq 5 : (assume_proof__ (assume___mul4_c0, assert___mul4_c0, assume_proof___mul4_c0, assert_proof___mul4_c0)). auto => />.
-    auto => />. 
+proc .
+wp -1 => /=. auto => />.
 qed.
 
-
-lemma __mul4_c1_assume  : hoare [M.__mul4_c1 : true ==> (assume_proof_ res)].
+lemma __mul4_c2_valid_post _h _r _f _g _z _cf _of :
+      hoare [M.__mul4_c2 :
+      ((_of = of_0) /\
+      ((_cf = cf) /\
+      ((_z = z) /\ ((_g = g) /\ ((_f = f) /\ ((_r = r) /\ (_h = h))))))) ==>
+      ((valid (trace res)) => true)].
 proof.
-    proc. 
-    seq 5 : (assume_proof__ (assume___mul4_c1, assert___mul4_c1, assume_proof___mul4_c1, assert_proof___mul4_c1)). auto => />.
-    auto => />. 
+proc .
+wp -1 => /=. auto => />.
 qed.
 
-lemma __mul4_c2_assume  : hoare [M.__mul4_c2 : true ==> (assume_proof_ res)].
+lemma __mul4_c3_valid_post _h _r _f _g _z _cf _of :
+      hoare [M.__mul4_c3 :
+      ((_of = of_0) /\
+      ((_cf = cf) /\
+      ((_z = z) /\ ((_g = g) /\ ((_f = f) /\ ((_r = r) /\ (_h = h))))))) ==>
+      ((valid (trace res)) => true)].
 proof.
-    proc. 
-    seq 5 : (assume_proof__ (assume___mul4_c2, assert___mul4_c2, assume_proof___mul4_c2, assert_proof___mul4_c2)). auto => />.
-    auto => />. 
+proc .
+wp -1 => /=. auto => />.
+qed .
+
+lemma __mul4_rsr_valid_post _fs _g :
+      hoare [M.__mul4_rsr :
+      ((_g = g) /\ (_fs = fs)) ==>
+      ((valid (trace res)) =>
+      (eqmod
+      (foldr (fun x => (fun (acc:int) => (x + acc))) 0
+      (map (fun ii => ((pow 2 (64 * ii)) * (u64i res.`1.[ii]))) (iota_ 0 4)))
+      ((foldr (fun x => (fun (acc:int) => (x + acc))) 0
+       (map (fun ii => ((pow 2 (64 * ii)) * (u64i _fs.[ii]))) (iota_ 0 4))) *
+      (foldr (fun x => (fun (acc:int) => (x + acc))) 0
+      (map (fun ii => ((pow 2 (64 * ii)) * (u64i _g.[ii]))) (iota_ 0 4))))
+      (single ((pow 2 255) - 19))))].
+proof.
+proc .
+wp -1 => /=.
+conseq (:  _ ==> ((_g = old_g) /\ (_fs = old_fs))).
+move => ? _ /> 2?.
+rewrite /trace /= valid_cat /valid //=.
+seq 2 : (((_g = old_g) /\ (_fs = old_fs))).
+by auto .
+by conseq  />.
+qed .
+
+(* The post is in the trace and all assumes are valid. *)
+
+lemma __reduce4_assume_ _x _r __38 _z _cf _of :
+      hoare [M.__reduce4 :
+      ((_of = of_0) /\
+      ((_cf = cf) /\ ((_z = z) /\ ((__38 = _38) /\ ((_r = r) /\ (_x = x)))))) ==>
+      (true => (validk Assume (trace res)))].
+proof.
+    proc. auto => />. move => H H0 H1. 
+    smt(@JUtils @Zp_25519 @Jcheck @W64).
 qed.
 
-lemma __mul4_c3_assume  : hoare [M.__mul4_c3 : true ==> (assume_proof_ res)].
+lemma __reduce4_assume _x _r __38 _z _cf _of :
+      hoare [M.__reduce4 :
+      ((_of = of_0) /\
+      ((_cf = cf) /\ ((_z = z) /\ ((__38 = _38) /\ ((_r = r) /\ (_x = x)))))) ==>
+      (((valid (trace res)) =>
+       (eqmod
+       (foldr (fun x => (fun (acc:int) => (x + acc))) 0
+       (map (fun ii => ((pow 2 (64 * ii)) * (u64i res.`1.[ii]))) (iota_ 0 4))
+       )
+       ((foldr (fun x => (fun (acc:int) => (x + acc))) 0
+        (map (fun ii => ((pow 2 (64 * ii)) * (u64i _x.[ii]))) (iota_ 0 4))) +
+       (foldr (fun x => (fun (acc:int) => (x + acc))) 0
+       (map (fun ii => ((pow 2 (64 * (ii + 4))) * (u64i _r.[ii])))
+       (iota_ 0 4)))) (single ((pow 2 255) - 19)))) /\
+      (true => (validk Assume (trace res))))].
 proof.
-    proc. 
-    seq 5 : (assume_proof__ (assume___mul4_c3, assert___mul4_c3, assume_proof___mul4_c3, assert_proof___mul4_c3)). auto => />.
-    auto => />. 
+conseq (__reduce4_assume_ _x _r __38 _z _cf _of) (__reduce4_valid_post 
+                                                  _x _r __38 _z _cf _of) 
+       => />.
+qed .
+
+lemma __mul4_c0_assume_ _f0 _g _z _cf _of :
+      hoare [M.__mul4_c0 :
+      ((_of = of_0) /\ ((_cf = cf) /\ ((_z = z) /\ ((_g = g) /\ (_f0 = f0))))) ==>
+      (true => (validk Assume (trace res)))].
+proof.
+    proc. auto => />.
 qed.
 
-lemma __mul4_rsr_assume  :
-      hoare [M.__mul4_rsr : true ==> (assume_proof_ res)].
+lemma __mul4_c0_assume _f0 _g _z _cf _of :
+      hoare [M.__mul4_c0 :
+      ((_of = of_0) /\ ((_cf = cf) /\ ((_z = z) /\ ((_g = g) /\ (_f0 = f0))))) ==>
+      (((valid (trace res)) => true) /\
+      (true => (validk Assume (trace res))))].
 proof.
-    proc.  
-    seq 8 : (assume_proof__ (assume___mul4_rsr, assert___mul4_rsr, assume_proof___mul4_rsr, assert_proof___mul4_rsr)). auto => />.
-    wp; call __reduce4_assume.
-    wp; call __mul4_c3_assume.
-    wp; call __mul4_c2_assume.
-    wp; call __mul4_c1_assume.
-    wp; call __mul4_c0_assume.
-    auto => />.
+conseq (__mul4_c0_assume_ _f0 _g _z _cf _of) (__mul4_c0_valid_post _f0 
+                                              _g _z _cf _of) => />.
+qed .
+
+lemma __mul4_c1_assume_ _h _r _f _g _z _cf _of :
+      hoare [M.__mul4_c1 :
+      ((_of = of_0) /\
+      ((_cf = cf) /\
+      ((_z = z) /\ ((_g = g) /\ ((_f = f) /\ ((_r = r) /\ (_h = h))))))) ==>
+      (true => (validk Assume (trace res)))].
+proof.
+    proc. auto => />.
 qed.
 
-(* Soundness of assert/assume. *)
-
-lemma __reduce4_assert_assume_sound  :
-      hoare [M.__reduce4 : true ==> (soundness_ res)].
+lemma __mul4_c1_assume _h _r _f _g _z _cf _of :
+      hoare [M.__mul4_c1 :
+      ((_of = of_0) /\
+      ((_cf = cf) /\
+      ((_z = z) /\ ((_g = g) /\ ((_f = f) /\ ((_r = r) /\ (_h = h))))))) ==>
+      (((valid (trace res)) => true) /\
+      (true => (validk Assume (trace res))))].
 proof.
-    proc.
-    seq 52 : (soundness__ (assume___reduce4, assert___reduce4, assume_proof___reduce4, assert_proof___reduce4)). auto => />. smt().
-    seq 23 : (soundness__ (assume___reduce4, assert___reduce4, assume_proof___reduce4, assert_proof___reduce4)). auto => />. smt().
-    auto => />. smt().
+conseq (__mul4_c1_assume_ _h _r _f _g _z _cf _of) (__mul4_c1_valid_post 
+                                                   _h _r _f _g _z _cf 
+                                                   _of) => />.
+qed .
+
+lemma __mul4_c2_assume_ _h _r _f _g _z _cf _of :
+      hoare [M.__mul4_c2 :
+      ((_of = of_0) /\
+      ((_cf = cf) /\
+      ((_z = z) /\ ((_g = g) /\ ((_f = f) /\ ((_r = r) /\ (_h = h))))))) ==>
+      (true => (validk Assume (trace res)))].
+proof.
+    proc. auto => />.
 qed.
 
-lemma __mul4_c0_assert_assume_sound  :
-      hoare [M.__mul4_c0 : true ==> (soundness_ res)].
+lemma __mul4_c2_assume _h _r _f _g _z _cf _of :
+      hoare [M.__mul4_c2 :
+      ((_of = of_0) /\
+      ((_cf = cf) /\
+      ((_z = z) /\ ((_g = g) /\ ((_f = f) /\ ((_r = r) /\ (_h = h))))))) ==>
+      (((valid (trace res)) => true) /\
+      (true => (validk Assume (trace res))))].
 proof.
- proc. 
- seq 5 : (soundness__ (assume___mul4_c0, assert___mul4_c0, assume_proof___mul4_c0, assert_proof___mul4_c0)). auto => />. auto => />. 
-  smt().
+conseq (__mul4_c2_assume_ _h _r _f _g _z _cf _of) (__mul4_c2_valid_post 
+                                                   _h _r _f _g _z _cf 
+                                                   _of) => />.
+qed .
+
+lemma __mul4_c3_assume_ _h _r _f _g _z _cf _of :
+      hoare [M.__mul4_c3 :
+      ((_of = of_0) /\
+      ((_cf = cf) /\
+      ((_z = z) /\ ((_g = g) /\ ((_f = f) /\ ((_r = r) /\ (_h = h))))))) ==>
+      (true => (validk Assume (trace res)))].
+proof.
+    proc. auto => />.
 qed.
 
-
-lemma __mul4_c1_assert_assume_sound  :
-      hoare [M.__mul4_c1 : true ==> (soundness_ res)].
+lemma __mul4_c3_assume _h _r _f _g _z _cf _of :
+      hoare [M.__mul4_c3 :
+      ((_of = of_0) /\
+      ((_cf = cf) /\
+      ((_z = z) /\ ((_g = g) /\ ((_f = f) /\ ((_r = r) /\ (_h = h))))))) ==>
+      (((valid (trace res)) => true) /\
+      (true => (validk Assume (trace res))))].
 proof.
- proc. 
- seq 5 : (soundness__ (assume___mul4_c1, assert___mul4_c1, assume_proof___mul4_c1, assert_proof___mul4_c1)). auto => />. auto => />. 
-  smt().
+conseq (__mul4_c3_assume_ _h _r _f _g _z _cf _of) (__mul4_c3_valid_post 
+                                                   _h _r _f _g _z _cf 
+                                                   _of) => />.
+qed .
+
+lemma __mul4_rsr_assume_ _fs _g :
+      hoare [M.__mul4_rsr :
+      ((_g = g) /\ (_fs = fs)) ==> (true => (validk Assume (trace res)))].
+proof.
+    proc. auto => />.
+    ecall (__reduce4_assume h r _38 z cf of_0). auto => />.
+    smt (valid_cat all_cat).
+    ecall (__mul4_c3_assume h r f g0 z cf of_0). auto => />.
+    ecall (__mul4_c2_assume h r f g0 z cf of_0). auto => />.
+    ecall (__mul4_c1_assume h r f g0 z cf of_0). auto => />.
+    ecall (__mul4_c0_assume f g0 z cf of_0). auto => />.
+    move => H H0 H1 H2 H3 H4 H5 H6 H7 H8 H9.
+    rewrite !/trace //= !validk_cat //=. 
+    rewrite !valid_cat //=. smt(forall_validk_valid).
 qed.
 
-lemma __mul4_c2_assert_assume_sound  :
-      hoare [M.__mul4_c2 : true ==> (soundness_ res)].
+lemma __mul4_rsr_assume _fs _g :
+      hoare [M.__mul4_rsr :
+      ((_g = g) /\ (_fs = fs)) ==>
+      (((valid (trace res)) =>
+       (eqmod
+       (foldr (fun x => (fun (acc:int) => (x + acc))) 0
+       (map (fun ii => ((pow 2 (64 * ii)) * (u64i res.`1.[ii]))) (iota_ 0 4))
+       )
+       ((foldr (fun x => (fun (acc:int) => (x + acc))) 0
+        (map (fun ii => ((pow 2 (64 * ii)) * (u64i _fs.[ii]))) (iota_ 0 4))) *
+       (foldr (fun x => (fun (acc:int) => (x + acc))) 0
+       (map (fun ii => ((pow 2 (64 * ii)) * (u64i _g.[ii]))) (iota_ 0 4))))
+       (single ((pow 2 255) - 19)))) /\
+      (true => (validk Assume (trace res))))].
 proof.
- proc. 
- seq 5 : (soundness__ (assume___mul4_c2, assert___mul4_c2, assume_proof___mul4_c2, assert_proof___mul4_c2)). auto => />. auto => />. 
-  smt().
-qed.
+conseq (__mul4_rsr_assume_ _fs _g) (__mul4_rsr_valid_post _fs _g) => />.
+qed .
 
-lemma __mul4_c3_assert_assume_sound  :
-      hoare [M.__mul4_c3 : true ==> (soundness_ res)].
-proof.
- proc. 
- seq 5 : (soundness__ (assume___mul4_c3, assert___mul4_c3, assume_proof___mul4_c3, assert_proof___mul4_c3)). auto => />. auto => />. 
-  smt().
-qed.
+(* All assert are valid. *)
 
-lemma __mul4_rsr_assert_assume_sound  :
-      hoare [M.__mul4_rsr : true ==> (soundness_ res)].
-proof.
-    proc.  
-    seq 8 : (soundness__ (assume___mul4_rsr, assert___mul4_rsr, assume_proof___mul4_rsr, assert_proof___mul4_rsr)). auto => />.
-    wp; call __reduce4_assert_assume_sound.
-    wp; call __mul4_c3_assert_assume_sound.
-    wp; call __mul4_c2_assert_assume_sound.
-    wp; call __mul4_c1_assert_assume_sound.
-    wp; call __mul4_c0_assert_assume_sound.
-    auto => />. smt().
-qed.
-
-(* Lemmas proved by cryptoline. *)
-
-(* of is a reserved keyword, rename to of_0 *)
-axiom __reduce4_assert _x _r __38 _z _cf _of :
+lemma __reduce4_assert _x _r __38 _z _cf _of :
       hoare [M.__reduce4 :
       (((_of = of_0) /\
        ((_cf = cf) /\ ((_z = z) /\ ((__38 = _38) /\ ((_r = r) /\ (_x = x)))))) /\
-      true) ==>
-      (_assert_spec res
-      (eqmod
-      (foldr (fun x => (fun (acc: int) => (x + acc))) 0
-      (map (fun ii => ((pow 2 (64 * ii)) * (u64i res.`1.[ii]))) (iota_ 0 4)))
-      ((foldr (fun x => (fun (acc: int) => (x + acc))) 0
-       (map (fun ii => ((pow 2 (64 * ii)) * (u64i _x.[ii]))) (iota_ 0 4))) +
-      (foldr (fun x => (fun (acc: int) => (x + acc))) 0
-      (map (fun ii => ((pow 2 (64 * (ii + 4))) * (u64i _r.[ii]))) (iota_ 0 4)
-      ))) (single ((pow 2 255) - 19))))].
+      true) ==> (validk Assert (trace res))].
+proof.
+admitted (* Proven by Cryptoline *).
 
-axiom __mul4_c0_assert _f0 _g _z _cf _of :
+lemma __mul4_c0_assert _f0 _g _z _cf _of :
       hoare [M.__mul4_c0 :
       (((_of = of_0) /\ ((_cf = cf) /\ ((_z = z) /\ ((_g = g) /\ (_f0 = f0))))) /\
-      true) ==> (_assert_spec res true)].
+      true) ==> (validk Assert (trace res))].
+proof.
+admitted (* Proven by Cryptoline *).
 
-axiom __mul4_c1_assert _h _r _f _g _z _cf _of :
+lemma __mul4_c1_assert _h _r _f _g _z _cf _of :
       hoare [M.__mul4_c1 :
       (((_of = of_0) /\
        ((_cf = cf) /\
        ((_z = z) /\ ((_g = g) /\ ((_f = f) /\ ((_r = r) /\ (_h = h))))))) /\
-      true) ==> (_assert_spec res true)].
+      true) ==> (validk Assert (trace res))].
+proof.
+admitted (* Proven by Cryptoline *).
 
-axiom __mul4_c2_assert _h _r _f _g _z _cf _of :
+lemma __mul4_c2_assert _h _r _f _g _z _cf _of :
       hoare [M.__mul4_c2 :
       (((_of = of_0) /\
        ((_cf = cf) /\
        ((_z = z) /\ ((_g = g) /\ ((_f = f) /\ ((_r = r) /\ (_h = h))))))) /\
-      true) ==> (_assert_spec res true)].
+      true) ==> (validk Assert (trace res))].
+proof.
+admitted (* Proven by Cryptoline *).
 
-axiom __mul4_c3_assert _h _r _f _g _z _cf _of :
+lemma __mul4_c3_assert _h _r _f _g _z _cf _of :
       hoare [M.__mul4_c3 :
       (((_of = of_0) /\
        ((_cf = cf) /\
        ((_z = z) /\ ((_g = g) /\ ((_f = f) /\ ((_r = r) /\ (_h = h))))))) /\
-      true) ==> (_assert_spec res true)].
+      true) ==> (validk Assert (trace res))].
+proof.
+admitted (* Proven by Cryptoline *).
 
-axiom __mul4_rsr_assert _fs _g :
+lemma __mul4_rsr_assert _fs _g :
       hoare [M.__mul4_rsr :
-      (((_g = g) /\ (_fs = fs)) /\ true) ==>
-      (_assert_spec res
-      (eqmod
-      (foldr (fun x => (fun (acc: int) => (x + acc))) 0
-      (map (fun ii => ((pow 2 (64 * ii)) * (u64i res.`1.[ii]))) (iota_ 0 4)))
-      ((foldr (fun x => (fun (acc: int) => (x + acc))) 0
-       (map (fun ii => ((pow 2 (64 * ii)) * (u64i _fs.[ii]))) (iota_ 0 4))) *
-      (foldr (fun x => (fun (acc: int) => (x + acc))) 0
-      (map (fun ii => ((pow 2 (64 * ii)) * (u64i _g.[ii]))) (iota_ 0 4))))
-      (single ((pow 2 255) - 19))))].
+      (((_g = g) /\ (_fs = fs)) /\ true) ==> (validk Assert (trace res))].
+proof.
+admitted (* Proven by Cryptoline *).
 
 (* Final specification for the functions. *)
 
-lemma __reduce4_spec  :
-      forall _x _r __38 _z _cf _of,
+lemma __reduce4_spec _x _r __38 _z _cf _of :
       hoare [M.__reduce4 :
       (((_of = of_0) /\
        ((_cf = cf) /\ ((_z = z) /\ ((__38 = _38) /\ ((_r = r) /\ (_x = x)))))) /\
       true) ==>
       (eqmod
-      (foldr (fun x => (fun (acc: int) => (x + acc))) 0
+      (foldr (fun x => (fun (acc:int) => (x + acc))) 0
       (map (fun ii => ((pow 2 (64 * ii)) * (u64i res.`1.[ii]))) (iota_ 0 4)))
-      ((foldr (fun x => (fun (acc: int) => (x + acc))) 0
+      ((foldr (fun x => (fun (acc:int) => (x + acc))) 0
        (map (fun ii => ((pow 2 (64 * ii)) * (u64i _x.[ii]))) (iota_ 0 4))) +
-      (foldr (fun x => (fun (acc: int) => (x + acc))) 0
+      (foldr (fun x => (fun (acc:int) => (x + acc))) 0
       (map (fun ii => ((pow 2 (64 * (ii + 4))) * (u64i _r.[ii]))) (iota_ 0 4)
       ))) (single ((pow 2 255) - 19)))].
 proof.
-move => _x _r __38 _z _cf _of.
-have h  :
-     hoare [M.__reduce4 :
-     (((_of = of_0) /\
-      ((_cf = cf) /\ ((_z = z) /\ ((__38 = _38) /\ ((_r = r) /\ (_x = x)))))) /\
-     true) ==>
-     (_spec_soundness res
-     (eqmod
-     (foldr (fun x => (fun (acc: int) => (x + acc))) 0
-     (map (fun ii => ((pow 2 (64 * ii)) * (u64i res.`1.[ii]))) (iota_ 0 4)))
-     ((foldr (fun x => (fun (acc: int) => (x + acc))) 0
-      (map (fun ii => ((pow 2 (64 * ii)) * (u64i _x.[ii]))) (iota_ 0 4))) +
-     (foldr (fun x => (fun (acc: int) => (x + acc))) 0
-     (map (fun ii => ((pow 2 (64 * (ii + 4))) * (u64i _r.[ii]))) (iota_ 0 4))
-     )) (single ((pow 2 255) - 19))))].
-by conseq __reduce4_assume (__reduce4_assert _x _r __38 _z _cf _of).
-conseq h __reduce4_assert_assume_sound => // ; smt ().
+conseq (__reduce4_assume _x _r __38 _z _cf _of) (__reduce4_assert _x 
+                                                 _r __38 _z _cf _of) 
+       => />.
+smt (all_validk_valid).
 qed .
 
-lemma __mul4_c0_spec  :
-      forall _f0 _g _z _cf _of,
+lemma __mul4_c0_spec _f0 _g _z _cf _of :
       hoare [M.__mul4_c0 :
       (((_of = of_0) /\ ((_cf = cf) /\ ((_z = z) /\ ((_g = g) /\ (_f0 = f0))))) /\
       true) ==> true].
 proof.
-move => _f0 _g _z _cf _of.
-have h  :
-     hoare [M.__mul4_c0 :
-     (((_of = of_0) /\ ((_cf = cf) /\ ((_z = z) /\ ((_g = g) /\ (_f0 = f0))))) /\
-     true) ==> (_spec_soundness res true)].
-by conseq __mul4_c0_assume (__mul4_c0_assert _f0 _g _z _cf _of).
-conseq h __mul4_c0_assert_assume_sound => // ; smt ().
+conseq (__mul4_c0_assume _f0 _g _z _cf _of) (__mul4_c0_assert _f0 _g 
+                                             _z _cf _of) => />.
 qed .
 
-lemma __mul4_c1_spec  :
-      forall _h _r _f _g _z _cf _of,
+lemma __mul4_c1_spec _h _r _f _g _z _cf _of :
       hoare [M.__mul4_c1 :
       (((_of = of_0) /\
        ((_cf = cf) /\
        ((_z = z) /\ ((_g = g) /\ ((_f = f) /\ ((_r = r) /\ (_h = h))))))) /\
       true) ==> true].
 proof.
-move => _h _r _f _g _z _cf _of.
-have h  :
-     hoare [M.__mul4_c1 :
-     (((_of = of_0) /\
-      ((_cf = cf) /\
-      ((_z = z) /\ ((_g = g) /\ ((_f = f) /\ ((_r = r) /\ (_h = h))))))) /\
-     true) ==> (_spec_soundness res true)].
-by conseq __mul4_c1_assume (__mul4_c1_assert _h _r _f _g _z _cf _of).
-conseq h __mul4_c1_assert_assume_sound => // ; smt ().
+conseq (__mul4_c1_assume _h _r _f _g _z _cf _of) (__mul4_c1_assert _h 
+                                                  _r _f _g _z _cf _of) 
+       => />.
 qed .
 
-lemma __mul4_c2_spec  :
-      forall _h _r _f _g _z _cf _of,
+lemma __mul4_c2_spec _h _r _f _g _z _cf _of :
       hoare [M.__mul4_c2 :
       (((_of = of_0) /\
        ((_cf = cf) /\
        ((_z = z) /\ ((_g = g) /\ ((_f = f) /\ ((_r = r) /\ (_h = h))))))) /\
       true) ==> true].
 proof.
-move => _h _r _f _g _z _cf _of.
-have h  :
-     hoare [M.__mul4_c2 :
-     (((_of = of_0) /\
-      ((_cf = cf) /\
-      ((_z = z) /\ ((_g = g) /\ ((_f = f) /\ ((_r = r) /\ (_h = h))))))) /\
-     true) ==> (_spec_soundness res true)].
-by conseq __mul4_c2_assume (__mul4_c2_assert _h _r _f _g _z _cf _of).
-conseq h __mul4_c2_assert_assume_sound => // ; smt ().
+conseq (__mul4_c2_assume _h _r _f _g _z _cf _of) (__mul4_c2_assert _h 
+                                                  _r _f _g _z _cf _of) 
+       => />.
 qed .
 
-lemma __mul4_c3_spec  :
-      forall _h _r _f _g _z _cf _of,
+lemma __mul4_c3_spec _h _r _f _g _z _cf _of :
       hoare [M.__mul4_c3 :
       (((_of = of_0) /\
        ((_cf = cf) /\
        ((_z = z) /\ ((_g = g) /\ ((_f = f) /\ ((_r = r) /\ (_h = h))))))) /\
       true) ==> true].
 proof.
-move => _h _r _f _g _z _cf _of.
-have h  :
-     hoare [M.__mul4_c3 :
-     (((_of = of_0) /\
-      ((_cf = cf) /\
-      ((_z = z) /\ ((_g = g) /\ ((_f = f) /\ ((_r = r) /\ (_h = h))))))) /\
-     true) ==> (_spec_soundness res true)].
-by conseq __mul4_c3_assume (__mul4_c3_assert _h _r _f _g _z _cf _of).
-conseq h __mul4_c3_assert_assume_sound => // ; smt ().
+conseq (__mul4_c3_assume _h _r _f _g _z _cf _of) (__mul4_c3_assert _h 
+                                                  _r _f _g _z _cf _of) 
+       => />.
 qed .
 
-lemma __mul4_rsr_spec  :
-      forall _fs _g,
+lemma __mul4_rsr_spec _fs _g :
       hoare [M.__mul4_rsr :
       (((_g = g) /\ (_fs = fs)) /\ true) ==>
       (eqmod
-      (foldr (fun x => (fun (acc: int) => (x + acc))) 0
+      (foldr (fun x => (fun (acc:int) => (x + acc))) 0
       (map (fun ii => ((pow 2 (64 * ii)) * (u64i res.`1.[ii]))) (iota_ 0 4)))
-      ((foldr (fun x => (fun (acc: int) => (x + acc))) 0
+      ((foldr (fun x => (fun (acc:int) => (x + acc))) 0
        (map (fun ii => ((pow 2 (64 * ii)) * (u64i _fs.[ii]))) (iota_ 0 4))) *
-      (foldr (fun x => (fun (acc: int) => (x + acc))) 0
+      (foldr (fun x => (fun (acc:int) => (x + acc))) 0
       (map (fun ii => ((pow 2 (64 * ii)) * (u64i _g.[ii]))) (iota_ 0 4))))
       (single ((pow 2 255) - 19)))].
 proof.
-move => _fs _g.
-have h  :
-     hoare [M.__mul4_rsr :
-     (((_g = g) /\ (_fs = fs)) /\ true) ==>
-     (_spec_soundness res
-     (eqmod
-     (foldr (fun x => (fun (acc: int) => (x + acc))) 0
-     (map (fun ii => ((pow 2 (64 * ii)) * (u64i res.`1.[ii]))) (iota_ 0 4)))
-     ((foldr (fun x => (fun (acc: int) => (x + acc))) 0
-      (map (fun ii => ((pow 2 (64 * ii)) * (u64i _fs.[ii]))) (iota_ 0 4))) *
-     (foldr (fun x => (fun (acc: int) => (x + acc))) 0
-     (map (fun ii => ((pow 2 (64 * ii)) * (u64i _g.[ii]))) (iota_ 0 4))))
-     (single ((pow 2 255) - 19))))].
-by conseq __mul4_rsr_assume (__mul4_rsr_assert _fs _g).
-conseq h __mul4_rsr_assert_assume_sound => // ; smt ().
+conseq (__mul4_rsr_assume _fs _g) (__mul4_rsr_assert _fs _g) => />.
+smt (all_validk_valid).
 qed .
