proof/crypto_scalarmult/curve25519/amd64/cryptoline_extraction/Mul4RefExtracted.ec
@@ -4,22 +4,23 @@ from Jasmin require import JModel_x86.
 
 import SLH64.
 
-require import Jcheck.
+from Jasmin require import Jcheck.
 
 require import Array4 Array8.
 
 require import WArray32 WArray64.
 
-require import Jcheck Zp_limbs Zp_25519 CommonCryptoline.
+require import Zp_limbs Zp_25519 CommonCryptoline.
 import Zp_25519 Zp Zp_limbs EClib.
 
+
 module M = {
-  var tmp__check : to_check
+  var tmp__trace : trace
   var tmp__data___reduce4 : (W64.t Array4.t)
   var tmp____reduce4 : W64.t Array4.t
   var tmp__data___mul4_rss : (W64.t Array4.t)
   var tmp____mul4_rss : W64.t Array4.t
-  proc __reduce4 (z:W64.t Array8.t) : ((W64.t Array4.t) * to_check) = {
+  proc __reduce4 (z:W64.t Array8.t) : ((W64.t Array4.t) * trace) = {
     var aux:bool;
     var aux_1:int;
     var aux_0:W64.t;
@@ -33,14 +34,10 @@ module M = {
     var i:int;
     var dc:W64.t;
     var r0:W64.t;
-    var assume___reduce4:bool;
-    var assert___reduce4:bool;
-    var assume_proof___reduce4:bool;
-    var assert_proof___reduce4:bool;
-    assume___reduce4 <- true;
-    assert___reduce4 <- true;
-    assume_proof___reduce4 <- true;
-    assert_proof___reduce4 <- assert___reduce4;
+    var old_z:W64.t Array8.t;
+    var trace___reduce4:trace;
+    old_z <- z;
+    trace___reduce4 <- [];
     r <- witness;
     r38 <- (W64.of_int 38);
     rax <- z.[4];
@@ -57,14 +54,8 @@ module M = {
     (aux, aux_0) <- (adc_64 r.[2] h cf);
     cf <- aux;
     r.[2] <- aux_0;
-    assert_proof___reduce4 <-
-    (assert_proof___reduce4 /\
-    ((assert___reduce4 /\ assume___reduce4) => (! cf)));
-    assert___reduce4 <- (assert___reduce4 /\ (! cf));
-    assume_proof___reduce4 <-
-    (assume_proof___reduce4 /\
-    ((assert___reduce4 /\ assume___reduce4) => ((b2i cf) = 0)));
-    assume___reduce4 <- (assume___reduce4 /\ ((b2i cf) = 0));
+    trace___reduce4 <- (trace___reduce4 ++ [(Assert, (! cf))]);
+    trace___reduce4 <- (trace___reduce4 ++ [(Assume, ((b2i cf) = 0))]);
     (h, l) <- (mulu_64 rax r38);
     (aux, aux_0) <- (adc_64 r.[2] l false);
     cf <- aux;
@@ -74,28 +65,16 @@ module M = {
     (aux, aux_0) <- (adc_64 r.[3] h cf);
     cf <- aux;
     r.[3] <- aux_0;
-    assert_proof___reduce4 <-
-    (assert_proof___reduce4 /\
-    ((assert___reduce4 /\ assume___reduce4) => (! cf)));
-    assert___reduce4 <- (assert___reduce4 /\ (! cf));
-    assume_proof___reduce4 <-
-    (assume_proof___reduce4 /\
-    ((assert___reduce4 /\ assume___reduce4) => ((b2i cf) = 0)));
-    assume___reduce4 <- (assume___reduce4 /\ ((b2i cf) = 0));
+    trace___reduce4 <- (trace___reduce4 ++ [(Assert, (! cf))]);
+    trace___reduce4 <- (trace___reduce4 ++ [(Assume, ((b2i cf) = 0))]);
     (h, l) <- (mulu_64 rax r38);
     (aux, aux_0) <- (adc_64 r.[3] l false);
     cf <- aux;
     r.[3] <- aux_0;
     z8 <- (MOV_64 (W64.of_int 0));
     (cf, z8) <- (adc_64 z8 h cf);
-    assert_proof___reduce4 <-
-    (assert_proof___reduce4 /\
-    ((assert___reduce4 /\ assume___reduce4) => (! cf)));
-    assert___reduce4 <- (assert___reduce4 /\ (! cf));
-    assume_proof___reduce4 <-
-    (assume_proof___reduce4 /\
-    ((assert___reduce4 /\ assume___reduce4) => ((b2i cf) = 0)));
-    assume___reduce4 <- (assume___reduce4 /\ ((b2i cf) = 0));
+    trace___reduce4 <- (trace___reduce4 ++ [(Assert, (! cf))]);
+    trace___reduce4 <- (trace___reduce4 ++ [(Assume, ((b2i cf) = 0))]);
     (aux, aux_0) <- (adc_64 r.[0] z.[0] false);
     cf <- aux;
     r.[0] <- aux_0;
@@ -107,23 +86,13 @@ module M = {
       i <- (i + 1);
     }
     (cf, z8) <- (adc_64 z8 (W64.of_int 0) cf);
-    assert_proof___reduce4 <-
-    (assert_proof___reduce4 /\
-    ((assert___reduce4 /\ assume___reduce4) => (! cf)));
-    assert___reduce4 <- (assert___reduce4 /\ (! cf));
-    assume_proof___reduce4 <-
-    (assume_proof___reduce4 /\
-    ((assert___reduce4 /\ assume___reduce4) => ((b2i cf) = 0)));
-    assume___reduce4 <- (assume___reduce4 /\ ((b2i cf) = 0));
+    trace___reduce4 <- (trace___reduce4 ++ [(Assert, (! cf))]);
+    trace___reduce4 <- (trace___reduce4 ++ [(Assume, ((b2i cf) = 0))]);
     (dc, z8) <- (mulu_64 z8 (W64.of_int 38));
-    assert_proof___reduce4 <-
-    (assert_proof___reduce4 /\
-    ((assert___reduce4 /\ assume___reduce4) => (dc = (W64.of_int 0))));
-    assert___reduce4 <- (assert___reduce4 /\ (dc = (W64.of_int 0)));
-    assume_proof___reduce4 <-
-    (assume_proof___reduce4 /\
-    ((assert___reduce4 /\ assume___reduce4) => (dc = (W64.of_int 0))));
-    assume___reduce4 <- (assume___reduce4 /\ (dc = (W64.of_int 0)));
+    trace___reduce4 <-
+    (trace___reduce4 ++ [(Assert, (dc = (W64.of_int 0)))]);
+    trace___reduce4 <-
+    (trace___reduce4 ++ [(Assume, (dc = (W64.of_int 0)))]);
     r0 <- (MOV_64 (W64.of_int 0));
     (aux, aux_0) <- (adc_64 r.[0] z8 false);
     cf <- aux;
@@ -136,70 +105,60 @@ module M = {
       i <- (i + 1);
     }
     (cf, r0) <- (adc_64 r0 r0 cf);
-    assert_proof___reduce4 <-
-    (assert_proof___reduce4 /\
-    ((assert___reduce4 /\ assume___reduce4) => (! cf)));
-    assert___reduce4 <- (assert___reduce4 /\ (! cf));
-    assume_proof___reduce4 <-
-    (assume_proof___reduce4 /\
-    ((assert___reduce4 /\ assume___reduce4) => ((b2i cf) = 0)));
-    assume___reduce4 <- (assume___reduce4 /\ ((b2i cf) = 0));
+    trace___reduce4 <- (trace___reduce4 ++ [(Assert, (! cf))]);
+    trace___reduce4 <- (trace___reduce4 ++ [(Assume, ((b2i cf) = 0))]);
     (dc, r0) <- (mulu_64 r0 (W64.of_int 38));
-    assert_proof___reduce4 <-
-    (assert_proof___reduce4 /\
-    ((assert___reduce4 /\ assume___reduce4) => (dc = (W64.of_int 0))));
-    assert___reduce4 <- (assert___reduce4 /\ (dc = (W64.of_int 0)));
-    assume_proof___reduce4 <-
-    (assume_proof___reduce4 /\
-    ((assert___reduce4 /\ assume___reduce4) => (dc = (W64.of_int 0))));
-    assume___reduce4 <- (assume___reduce4 /\ (dc = (W64.of_int 0)));
+    trace___reduce4 <-
+    (trace___reduce4 ++ [(Assert, (dc = (W64.of_int 0)))]);
+    trace___reduce4 <-
+    (trace___reduce4 ++ [(Assume, (dc = (W64.of_int 0)))]);
     (aux, aux_0) <- (adc_64 r.[0] r0 false);
     cf <- aux;
     r.[0] <- aux_0;
-    assert_proof___reduce4 <-
-    (assert_proof___reduce4 /\
-    ((assert___reduce4 /\ assume___reduce4) => (! cf)));
-    assert___reduce4 <- (assert___reduce4 /\ (! cf));
-    assume_proof___reduce4 <-
-    (assume_proof___reduce4 /\
-    ((assert___reduce4 /\ assume___reduce4) => ((b2i cf) = 0)));
-    assume___reduce4 <- (assume___reduce4 /\ ((b2i cf) = 0));
-    return (r,
-           (assume___reduce4, assert___reduce4, assume_proof___reduce4,
-           assert_proof___reduce4));
+    trace___reduce4 <- (trace___reduce4 ++ [(Assert, (! cf))]);
+    trace___reduce4 <- (trace___reduce4 ++ [(Assume, ((b2i cf) = 0))]);
+    trace___reduce4 <-
+    (trace___reduce4 ++
+    [(Assert,
+     (eqmod
+     (foldr (fun x => (fun (acc:int) => (x + acc))) 0
+     (map (fun ii => ((pow 2 (64 * ii)) * (u64i r.[ii]))) (iota_ 0 4)))
+     (foldr (fun x => (fun (acc:int) => (x + acc))) 0
+     (map (fun ii => ((pow 2 (64 * ii)) * (u64i old_z.[ii]))) (iota_ 0 8)))
+     (single ((pow 2 255) - 19))))]);
+    return (r, trace___reduce4);
   }
   proc __mul4_rss (xa:W64.t Array4.t, ya:W64.t Array4.t) : ((W64.t Array4.t) *
-                                                           to_check) = {
+                                                           trace) = {
     var aux_0:bool;
     var aux:int;
     var aux_1:W64.t;
     var r:W64.t Array4.t;
     var i:int;
     var z:W64.t Array8.t;
+    var hprev:W64.t;
     var x:W64.t Array4.t;
     var j:int;
     var y:W64.t Array4.t;
     var h:W64.t;
     var l:W64.t;
     var cf:bool;
-    var hprev:W64.t;
-    var assume___mul4_rss:bool;
-    var assert___mul4_rss:bool;
-    var assume_proof___mul4_rss:bool;
-    var assert_proof___mul4_rss:bool;
-    assume___mul4_rss <- true;
-    assert___mul4_rss <- true;
-    assume_proof___mul4_rss <- true;
-    assert_proof___mul4_rss <- assert___mul4_rss;
+    var old_ya:W64.t Array4.t;
+    var old_xa:W64.t Array4.t;
+    var trace___mul4_rss:trace;
+    old_xa <- xa;
+    old_ya <- ya;
+    trace___mul4_rss <- [];
     r <- witness;
     x <- witness;
     y <- witness;
     z <- witness;
-    i <- 2;
+    i <- 0;
     while ((i < 8)) {
       z.[i] <- (MOV_64 (W64.of_int 0));
       i <- (i + 1);
     }
+    hprev <- (MOV_64 (W64.of_int 0));
     x.[0] <- xa.[0];
     j <- 0;
     while ((j < 4)) {
@@ -215,14 +174,8 @@ module M = {
         (aux_0, aux_1) <- (adc_64 z.[(j + 1)] h cf);
         cf <- aux_0;
         z.[(j + 1)] <- aux_1;
-        assert_proof___mul4_rss <-
-        (assert_proof___mul4_rss /\
-        ((assert___mul4_rss /\ assume___mul4_rss) => (! cf)));
-        assert___mul4_rss <- (assert___mul4_rss /\ (! cf));
-        assume_proof___mul4_rss <-
-        (assume_proof___mul4_rss /\
-        ((assert___mul4_rss /\ assume___mul4_rss) => ((b2i cf) = 0)));
-        assume___mul4_rss <- (assume___mul4_rss /\ ((b2i cf) = 0));
+        trace___mul4_rss <- (trace___mul4_rss ++ [(Assert, (! cf))]);
+        trace___mul4_rss <- (trace___mul4_rss ++ [(Assume, ((b2i cf) = 0))]);
       }
       j <- (j + 1);
     }
@@ -239,259 +192,228 @@ module M = {
         if ((j = 0)) {
           hprev <- (MOV_64 (W64.of_int 0));
           (cf, hprev) <- (adc_64 hprev h cf);
-          assert_proof___mul4_rss <-
-          (assert_proof___mul4_rss /\
-          ((assert___mul4_rss /\ assume___mul4_rss) => (! cf)));
-          assert___mul4_rss <- (assert___mul4_rss /\ (! cf));
-          assume_proof___mul4_rss <-
-          (assume_proof___mul4_rss /\
-          ((assert___mul4_rss /\ assume___mul4_rss) => ((b2i cf) = 0)));
-          assume___mul4_rss <- (assume___mul4_rss /\ ((b2i cf) = 0));
+          trace___mul4_rss <- (trace___mul4_rss ++ [(Assert, (! cf))]);
+          trace___mul4_rss <-
+          (trace___mul4_rss ++ [(Assume, ((b2i cf) = 0))]);
         } else {
           (cf, h) <- (adc_64 h (W64.of_int 0) cf);
-          assert_proof___mul4_rss <-
-          (assert_proof___mul4_rss /\
-          ((assert___mul4_rss /\ assume___mul4_rss) => (! cf)));
-          assert___mul4_rss <- (assert___mul4_rss /\ (! cf));
-          assume_proof___mul4_rss <-
-          (assume_proof___mul4_rss /\
-          ((assert___mul4_rss /\ assume___mul4_rss) => ((b2i cf) = 0)));
-          assume___mul4_rss <- (assume___mul4_rss /\ ((b2i cf) = 0));
+          trace___mul4_rss <- (trace___mul4_rss ++ [(Assert, (! cf))]);
+          trace___mul4_rss <-
+          (trace___mul4_rss ++ [(Assume, ((b2i cf) = 0))]);
           (aux_0, aux_1) <- (adc_64 z.[(i + j)] hprev false);
           cf <- aux_0;
           z.[(i + j)] <- aux_1;
           if (((1 <= j) /\ (j < (4 - 1)))) {
             hprev <- (MOV_64 (W64.of_int 0));
             (cf, hprev) <- (adc_64 hprev h cf);
-            assert_proof___mul4_rss <-
-            (assert_proof___mul4_rss /\
-            ((assert___mul4_rss /\ assume___mul4_rss) => (! cf)));
-            assert___mul4_rss <- (assert___mul4_rss /\ (! cf));
-            assume_proof___mul4_rss <-
-            (assume_proof___mul4_rss /\
-            ((assert___mul4_rss /\ assume___mul4_rss) => ((b2i cf) = 0)));
-            assume___mul4_rss <- (assume___mul4_rss /\ ((b2i cf) = 0));
+            trace___mul4_rss <- (trace___mul4_rss ++ [(Assert, (! cf))]);
+            trace___mul4_rss <-
+            (trace___mul4_rss ++ [(Assume, ((b2i cf) = 0))]);
           } else {
             (aux_0, aux_1) <- (adc_64 z.[((i + j) + 1)] h cf);
             cf <- aux_0;
             z.[((i + j) + 1)] <- aux_1;
-            assert_proof___mul4_rss <-
-            (assert_proof___mul4_rss /\
-            ((assert___mul4_rss /\ assume___mul4_rss) => (! cf)));
-            assert___mul4_rss <- (assert___mul4_rss /\ (! cf));
-            assume_proof___mul4_rss <-
-            (assume_proof___mul4_rss /\
-            ((assert___mul4_rss /\ assume___mul4_rss) => ((b2i cf) = 0)));
-            assume___mul4_rss <- (assume___mul4_rss /\ ((b2i cf) = 0));
+            trace___mul4_rss <- (trace___mul4_rss ++ [(Assert, (! cf))]);
+            trace___mul4_rss <-
+            (trace___mul4_rss ++ [(Assume, ((b2i cf) = 0))]);
           }
         }
         j <- (j + 1);
       }
       i <- (i + 1);
     }
-    (tmp__data___reduce4, tmp__check) <@ __reduce4 (z);
+    (tmp__data___reduce4, tmp__trace) <@ __reduce4 (z);
     tmp____reduce4 <- tmp__data___reduce4;
-    (assume___mul4_rss, assert___mul4_rss, assume_proof___mul4_rss,
-    assert_proof___mul4_rss) <-
-    (upd_call
-    (assume___mul4_rss, assert___mul4_rss, assume_proof___mul4_rss,
-    assert_proof___mul4_rss) tmp__check);
-    assert_proof___mul4_rss <-
-    (assert_proof___mul4_rss /\
-    ((assert___mul4_rss /\ assume___mul4_rss) =>
-    (eqmod
-    (foldr (fun x => (fun (acc: int) => (x + acc))) 0
-    (map (fun ii => ((pow 2 (64 * ii)) * (u64i tmp____reduce4.[ii])))
-    (iota_ 0 4)))
-    (foldr (fun x => (fun (acc: int) => (x + acc))) 0
-    (map (fun ii => ((pow 2 (64 * ii)) * (u64i z.[ii]))) (iota_ 0 8)))
-    (single ((pow 2 255) - 19)))));
-    assert___mul4_rss <-
-    (assert___mul4_rss /\
-    (eqmod
-    (foldr (fun x => (fun (acc: int) => (x + acc))) 0
-    (map (fun ii => ((pow 2 (64 * ii)) * (u64i tmp____reduce4.[ii])))
-    (iota_ 0 4)))
-    (foldr (fun x => (fun (acc: int) => (x + acc))) 0
-    (map (fun ii => ((pow 2 (64 * ii)) * (u64i z.[ii]))) (iota_ 0 8)))
-    (single ((pow 2 255) - 19))));
+    trace___mul4_rss <- (trace___mul4_rss ++ tmp__trace);
+    trace___mul4_rss <-
+    (trace___mul4_rss ++
+    [(Assume,
+     (eqmod
+     (foldr (fun x => (fun (acc:int) => (x + acc))) 0
+     (map (fun ii => ((pow 2 (64 * ii)) * (u64i tmp____reduce4.[ii])))
+     (iota_ 0 4)))
+     (foldr (fun x => (fun (acc:int) => (x + acc))) 0
+     (map (fun ii => ((pow 2 (64 * ii)) * (u64i z.[ii]))) (iota_ 0 8)))
+     (single ((pow 2 255) - 19))))]);
     r <- tmp____reduce4;
-    return (r,
-           (assume___mul4_rss, assert___mul4_rss, assume_proof___mul4_rss,
-           assert_proof___mul4_rss));
+    trace___mul4_rss <-
+    (trace___mul4_rss ++
+    [(Assert,
+     (eqmod
+     (foldr (fun x => (fun (acc:int) => (x + acc))) 0
+     (map (fun ii => ((pow 2 (64 * ii)) * (u64i r.[ii]))) (iota_ 0 4)))
+     ((foldr (fun x => (fun (acc:int) => (x + acc))) 0
+      (map (fun ii => ((pow 2 (64 * ii)) * (u64i old_xa.[ii]))) (iota_ 0 4))) *
+     (foldr (fun x => (fun (acc:int) => (x + acc))) 0
+     (map (fun ii => ((pow 2 (64 * ii)) * (u64i old_ya.[ii]))) (iota_ 0 4))))
+     (single ((pow 2 255) - 19))))]);
+    return (r, trace___mul4_rss);
   }
 }.
+(* The post is in the trace. *)
 
-(* All assume are valid. *)
-
-lemma __reduce4_assume  : hoare [M.__reduce4 : true ==> (assume_proof_ res)].
-proof.
-    proc. 
-     seq 21 : (assume_proof__ (assume___reduce4, assert___reduce4, assume_proof___reduce4, assert_proof___reduce4)). auto => />.
-     seq 13 : (assume_proof__ (assume___reduce4, assert___reduce4, assume_proof___reduce4, assert_proof___reduce4)). auto => />.
-     seq 16 : (assume_proof__ (assume___reduce4, assert___reduce4, assume_proof___reduce4, assert_proof___reduce4)). auto => />.
-     seq 12 : (assume_proof__ (assume___reduce4, assert___reduce4, assume_proof___reduce4, assert_proof___reduce4)). auto => />. auto => />.
-     seq 7 : (assume_proof__ (assume___reduce4, assert___reduce4, assume_proof___reduce4, assert_proof___reduce4)). auto => />. auto => />.
-     auto => />.
-qed.
-lemma __mul4_rss_assume  :
-      hoare [M.__mul4_rss : true ==> (assume_proof_ res)].
-proof.
-    proc. wp. call __reduce4_assume.
-    seq 8 : (assume_proof__ (assume___mul4_rss, assert___mul4_rss, assume_proof___mul4_rss,
-      assert_proof___mul4_rss)). auto => />.
-    unroll for ^while. auto => />. auto => />. auto => />. 
-    seq 14 : (assume_proof__ (assume___mul4_rss, assert___mul4_rss, assume_proof___mul4_rss,
-      assert_proof___mul4_rss)). auto => />.
-    seq 2 : (assume_proof__ (assume___mul4_rss, assert___mul4_rss, assume_proof___mul4_rss,
-      assert_proof___mul4_rss)). 
-    unroll for ^while. auto => />.
-    seq 2 : (assume_proof__ (assume___mul4_rss, assert___mul4_rss, assume_proof___mul4_rss,
-      assert_proof___mul4_rss)). 
-    unroll for ^while. auto => />. 
-    seq 5 : (assume_proof__ (assume___mul4_rss, assert___mul4_rss, assume_proof___mul4_rss,
-      assert_proof___mul4_rss)). 
-    unroll for ^while. auto => />.
-    seq 5 : (assume_proof__ (assume___mul4_rss, assert___mul4_rss, assume_proof___mul4_rss,
-      assert_proof___mul4_rss)). 
-    unroll for ^while. 
-    rcondt ^if. auto => />. rcondf ^if. auto => />. rcondt ^if. auto => />.
-    rcondf ^if. auto => />. rcondt ^if. auto => />. rcondf ^if. auto => />.
-    rcondf ^if. auto => />. auto => />. 
-    unroll for ^while. 
-    rcondt ^if. auto => />. rcondf ^if. auto => />. rcondt ^if. auto => />.
-    rcondf ^if. auto => />. rcondt ^if. auto => />. rcondf ^if. auto => />.
-    rcondf ^if. auto => />. auto => />. 
-    auto => />. 
-qed.
-    
-(* Soundness of assert/assume. *)
-
-lemma __reduce4_assert_assume_sound  :
-      hoare [M.__reduce4 : true ==> (soundness_ res)].
-proof.
-    proc.
-    seq 20: ( soundness__ (assume___reduce4, assert___reduce4, assume_proof___reduce4, assert_proof___reduce4)). auto => />.
-    seq 18: ( soundness__ (assume___reduce4, assert___reduce4, assume_proof___reduce4, assert_proof___reduce4)). auto => />. smt().
-    seq 12: ( soundness__ (assume___reduce4, assert___reduce4, assume_proof___reduce4, assert_proof___reduce4)). auto => />. smt(). 
-    seq 3: ( soundness__ (assume___reduce4, assert___reduce4, assume_proof___reduce4, assert_proof___reduce4)). auto => />. auto => />.
-    seq 13: ( soundness__ (assume___reduce4, assert___reduce4, assume_proof___reduce4, assert_proof___reduce4)). auto => />. smt().
-    seq 3: ( soundness__ (assume___reduce4, assert___reduce4, assume_proof___reduce4, assert_proof___reduce4)). auto => />. auto => />.
-    auto => />. smt().
-qed.
-
-lemma __mul4_rss_assert_assume_sound  :
-      hoare [M.__mul4_rss : true ==> (soundness_ res)].
-proof.
-    proc. wp. call __reduce4_assert_assume_sound.        
-    seq 8 : (soundness__ (assume___mul4_rss, assert___mul4_rss, assume_proof___mul4_rss,
-      assert_proof___mul4_rss)). auto => />.
-    unroll for ^while. auto => />. auto => />. auto => />. 
-    seq 14 : (soundness__ (assume___mul4_rss, assert___mul4_rss, assume_proof___mul4_rss,
-      assert_proof___mul4_rss)). auto => />.
-    seq 2 : (soundness__ (assume___mul4_rss, assert___mul4_rss, assume_proof___mul4_rss,
-      assert_proof___mul4_rss)). 
-    unroll for ^while. auto => />. smt().
-    seq 2 : (soundness__ (assume___mul4_rss, assert___mul4_rss, assume_proof___mul4_rss,
-      assert_proof___mul4_rss)). 
-    unroll for ^while. auto => />. 
-    seq 5 : (soundness__ (assume___mul4_rss, assert___mul4_rss, assume_proof___mul4_rss,
-      assert_proof___mul4_rss)). 
-    unroll for ^while. auto => />. smt().
-    seq 5 : (soundness__ (assume___mul4_rss, assert___mul4_rss, assume_proof___mul4_rss,
-      assert_proof___mul4_rss)). 
-    unroll for ^while. 
-    rcondt ^if. auto => />. rcondf ^if. auto => />. rcondt ^if. auto => />.
-    rcondf ^if. auto => />. rcondt ^if. auto => />. rcondf ^if. auto => />.
-    rcondf ^if. auto => />. wp. skip. auto => />. smt().
-    unroll for ^while. 
-    rcondt ^if. auto => />. rcondf ^if. auto => />. rcondt ^if. auto => />.
-    rcondf ^if. auto => />. rcondt ^if. auto => />. rcondf ^if. auto => />.
-    rcondf ^if. auto => />. wp. skip. auto => />. smt(). 
-    auto => />. smt().
-qed.
-
-(* Lemmas proved by cryptoline. *)
-
-axiom __reduce4_assert _z :
+lemma __reduce4_valid_post _z :
       hoare [M.__reduce4 :
-      ((_z = z) /\ true) ==>
-      (_assert_spec res
+      (_z = z) ==>
+      ((valid (trace res)) =>
       (eqmod
-      (foldr (fun x => (fun (acc: int) => (x + acc))) 0
+      (foldr (fun x => (fun (acc:int) => (x + acc))) 0
       (map (fun ii => ((pow 2 (64 * ii)) * (u64i res.`1.[ii]))) (iota_ 0 4)))
-      (foldr (fun x => (fun (acc: int) => (x + acc))) 0
+      (foldr (fun x => (fun (acc:int) => (x + acc))) 0
       (map (fun ii => ((pow 2 (64 * ii)) * (u64i _z.[ii]))) (iota_ 0 8)))
       (single ((pow 2 255) - 19))))].
+proof.
+proc .
+wp -1 => /=.
+conseq (:  _ ==> (_z = old_z)).
+move => ? _ /> 2?.
+rewrite /trace /= valid_cat /valid //=.
+seq 1 : ((_z = old_z)).
+by auto .
+by conseq  />.
+qed .
 
-axiom __mul4_rss_assert _xa _ya :
+lemma __mul4_rss_valid_post _xa _ya :
       hoare [M.__mul4_rss :
-      (((_ya = ya) /\ (_xa = xa)) /\ true) ==>
-      (_assert_spec res
+      ((_ya = ya) /\ (_xa = xa)) ==>
+      ((valid (trace res)) =>
       (eqmod
-      (foldr (fun x => (fun (acc: int) => (x + acc))) 0
+      (foldr (fun x => (fun (acc:int) => (x + acc))) 0
       (map (fun ii => ((pow 2 (64 * ii)) * (u64i res.`1.[ii]))) (iota_ 0 4)))
-      ((foldr (fun x => (fun (acc: int) => (x + acc))) 0
+      ((foldr (fun x => (fun (acc:int) => (x + acc))) 0
        (map (fun ii => ((pow 2 (64 * ii)) * (u64i _xa.[ii]))) (iota_ 0 4))) *
-      (foldr (fun x => (fun (acc: int) => (x + acc))) 0
+      (foldr (fun x => (fun (acc:int) => (x + acc))) 0
       (map (fun ii => ((pow 2 (64 * ii)) * (u64i _ya.[ii]))) (iota_ 0 4))))
       (single ((pow 2 255) - 19))))].
+proof.
+proc .
+wp -1 => /=.
+conseq (:  _ ==> ((_ya = old_ya) /\ (_xa = old_xa))).
+move => ? _ /> 2?.
+rewrite /trace /= valid_cat /valid //=.
+seq 2 : (((_ya = old_ya) /\ (_xa = old_xa))).
+by auto .
+by conseq  />.
+qed .
+
+(* The post is in the trace and all assumes are valid. *)
+
+lemma __reduce4_assume_ _z :
+      hoare [M.__reduce4 :
+      (_z = z) ==> (true => (validk Assume (trace res)))].
+proof.
+    proc. do 2! unroll for ^while. 
+    auto => />.
+qed.
+
+lemma __reduce4_assume _z :
+      hoare [M.__reduce4 :
+      (_z = z) ==>
+      (((valid (trace res)) =>
+       (eqmod
+       (foldr (fun x => (fun (acc:int) => (x + acc))) 0
+       (map (fun ii => ((pow 2 (64 * ii)) * (u64i res.`1.[ii]))) (iota_ 0 4))
+       )
+       (foldr (fun x => (fun (acc:int) => (x + acc))) 0
+       (map (fun ii => ((pow 2 (64 * ii)) * (u64i _z.[ii]))) (iota_ 0 8)))
+       (single ((pow 2 255) - 19)))) /\
+      (true => (validk Assume (trace res))))].
+proof.
+conseq (__reduce4_assume_ _z) (__reduce4_valid_post _z) => />.
+qed .
+
+lemma __mul4_rss_assume_ _xa _ya :
+      hoare [M.__mul4_rss :
+      ((_ya = ya) /\ (_xa = xa)) ==> (true => (validk Assume (trace res)))].
+proof.
+    proc. wp. 
+    seq 3: (#pre /\ validk Assume (trace___mul4_rss)). auto => />.  
+    seq 8: (#pre). unroll for ^while.  auto => />.  
+    seq 2: (#pre). unroll for ^while.   
+    rcondt ^if. auto. rcondf ^if. auto. rcondf ^if. auto. rcondf ^if. auto. auto => />.
+    move => &hr H. rewrite !validk_cat //=; 1..3:smt(@Jcheck @W64 @JUtils). 
+    seq 2: (#pre). unroll for ^while.   
+    seq 3: (#pre). unroll for ^while.   
+    rcondt ^if. auto. rcondf ^if. auto. rcondt ^if. auto. rcondf ^if. auto. rcondt ^if. auto. 
+    rcondf ^if. auto. rcondf ^if. auto. auto => />.  
+    move => &hr H. rewrite !validk_cat //=; 1..7:smt(@Jcheck @W64 @JUtils).
+    seq 3: (#pre). unroll for ^while.   
+    rcondt ^if. auto. rcondf ^if. auto. rcondt ^if. auto. rcondf ^if. auto. rcondt ^if. auto. 
+    rcondf ^if. auto. rcondf ^if. auto. auto => />.
+    move => &hr H. rewrite !validk_cat //=; 1..7:smt(@Jcheck @W64 @JUtils).
+    seq 3: (#pre). unroll for ^while.   
+    rcondt ^if. auto. rcondf ^if. auto. rcondt ^if. auto. rcondf ^if. auto. rcondt ^if. auto. 
+    rcondf ^if. auto. rcondf ^if. auto. auto => />.
+    move => &hr H. rewrite !validk_cat //=; 1..7:smt(@Jcheck @W64 @JUtils).
+    auto. inline M.__reduce4. 
+    do 2! unroll for ^while. 
+    auto => />.
+    move => &hr H. rewrite !/trace //= !validk_cat //=. move => H0 H1.
+    rewrite !H1 !b2i0 => />. rewrite !valid_cat //=. smt(forall_validk_valid).
+qed.
+
+
+lemma __mul4_rss_assume _xa _ya :
+      hoare [M.__mul4_rss :
+      ((_ya = ya) /\ (_xa = xa)) ==>
+      (((valid (trace res)) =>
+       (eqmod
+       (foldr (fun x => (fun (acc:int) => (x + acc))) 0
+       (map (fun ii => ((pow 2 (64 * ii)) * (u64i res.`1.[ii]))) (iota_ 0 4))
+       )
+       ((foldr (fun x => (fun (acc:int) => (x + acc))) 0
+        (map (fun ii => ((pow 2 (64 * ii)) * (u64i _xa.[ii]))) (iota_ 0 4))) *
+       (foldr (fun x => (fun (acc:int) => (x + acc))) 0
+       (map (fun ii => ((pow 2 (64 * ii)) * (u64i _ya.[ii]))) (iota_ 0 4))))
+       (single ((pow 2 255) - 19)))) /\
+      (true => (validk Assume (trace res))))].
+proof.
+conseq (__mul4_rss_assume_ _xa _ya) (__mul4_rss_valid_post _xa _ya) => />.
+qed .
+
+(* All assert are valid. *)
+
+lemma __reduce4_assert _z :
+      hoare [M.__reduce4 :
+      ((_z = z) /\ true) ==> (validk Assert (trace res))].
+proof.
+admitted (* Proven by Cryptoline *).
+
+lemma __mul4_rss_assert _xa _ya :
+      hoare [M.__mul4_rss :
+      (((_ya = ya) /\ (_xa = xa)) /\ true) ==> (validk Assert (trace res))].
+proof.
+admitted (* Proven by Cryptoline *).
 
 (* Final specification for the functions. *)
 
-lemma __reduce4_spec  :
-      forall _z,
+lemma __reduce4_spec _z :
       hoare [M.__reduce4 :
       ((_z = z) /\ true) ==>
       (eqmod
-      (foldr (fun x => (fun (acc: int) => (x + acc))) 0
+      (foldr (fun x => (fun (acc:int) => (x + acc))) 0
       (map (fun ii => ((pow 2 (64 * ii)) * (u64i res.`1.[ii]))) (iota_ 0 4)))
-      (foldr (fun x => (fun (acc: int) => (x + acc))) 0
+      (foldr (fun x => (fun (acc:int) => (x + acc))) 0
       (map (fun ii => ((pow 2 (64 * ii)) * (u64i _z.[ii]))) (iota_ 0 8)))
       (single ((pow 2 255) - 19)))].
 proof.
-move => _z.
-have h  :
-     hoare [M.__reduce4 :
-     ((_z = z) /\ true) ==>
-     (_spec_soundness res
-     (eqmod
-     (foldr (fun x => (fun (acc: int) => (x + acc))) 0
-     (map (fun ii => ((pow 2 (64 * ii)) * (u64i res.`1.[ii]))) (iota_ 0 4)))
-     (foldr (fun x => (fun (acc: int) => (x + acc))) 0
-     (map (fun ii => ((pow 2 (64 * ii)) * (u64i _z.[ii]))) (iota_ 0 8)))
-     (single ((pow 2 255) - 19))))].
-by conseq __reduce4_assume (__reduce4_assert _z).
-conseq h __reduce4_assert_assume_sound => // ; smt ().
-qed.
+conseq (__reduce4_assume _z) (__reduce4_assert _z) => />.
+smt (all_validk_valid).
+qed .
 
-lemma __mul4_rss_spec  :
-      forall _xa _ya,
+lemma __mul4_rss_spec _xa _ya :
       hoare [M.__mul4_rss :
       (((_ya = ya) /\ (_xa = xa)) /\ true) ==>
       (eqmod
-      (foldr (fun x => (fun (acc: int) => (x + acc))) 0
+      (foldr (fun x => (fun (acc:int) => (x + acc))) 0
       (map (fun ii => ((pow 2 (64 * ii)) * (u64i res.`1.[ii]))) (iota_ 0 4)))
-      ((foldr (fun x => (fun (acc: int) => (x + acc))) 0
+      ((foldr (fun x => (fun (acc:int) => (x + acc))) 0
        (map (fun ii => ((pow 2 (64 * ii)) * (u64i _xa.[ii]))) (iota_ 0 4))) *
-      (foldr (fun x => (fun (acc: int) => (x + acc))) 0
+      (foldr (fun x => (fun (acc:int) => (x + acc))) 0
       (map (fun ii => ((pow 2 (64 * ii)) * (u64i _ya.[ii]))) (iota_ 0 4))))
       (single ((pow 2 255) - 19)))].
 proof.
-move => _xa _ya.
-have h  :
-     hoare [M.__mul4_rss :
-     (((_ya = ya) /\ (_xa = xa)) /\ true) ==>
-     (_spec_soundness res
-     (eqmod
-     (foldr (fun x => (fun (acc: int) => (x + acc))) 0
-     (map (fun ii => ((pow 2 (64 * ii)) * (u64i res.`1.[ii]))) (iota_ 0 4)))
-     ((foldr (fun x => (fun (acc: int) => (x + acc))) 0
-      (map (fun ii => ((pow 2 (64 * ii)) * (u64i _xa.[ii]))) (iota_ 0 4))) *
-     (foldr (fun x => (fun (acc: int) => (x + acc))) 0
-     (map (fun ii => ((pow 2 (64 * ii)) * (u64i _ya.[ii]))) (iota_ 0 4))))
-     (single ((pow 2 255) - 19))))].
-by conseq __mul4_rss_assume (__mul4_rss_assert _xa _ya).
-conseq h __mul4_rss_assert_assume_sound => // ; smt ().
+conseq (__mul4_rss_assume _xa _ya) (__mul4_rss_assert _xa _ya) => />.
+smt (all_validk_valid).
 qed .
 
