proof/crypto_scalarmult/curve25519/amd64/cryptoline_extraction/Mul4_a24MulxExtracted.ec
@@ -1,23 +1,23 @@
-require import Int AllCore IntDiv CoreMap List Distr.
+require import AllCore IntDiv CoreMap List Distr.
 
 from Jasmin require import JModel_x86.
 
 import SLH64.
 
-require import Jcheck.
+from Jasmin require import Jcheck.
 
 require import Array4.
 
 require import WArray32.
 
-require import Jcheck Zp_limbs Zp_25519 CommonCryptoline.
+require import Zp_limbs Zp_25519 CommonCryptoline.
 import Zp_25519 Zp Zp_limbs EClib.
 
 module M = {
-  var tmp__check : to_check
+  var tmp__trace : trace
   var tmp__data___mul4_a24_rs : (W64.t Array4.t)
   var tmp____mul4_a24_rs : W64.t Array4.t
-  proc __mul4_a24_rs (fs:W64.t Array4.t) : ((W64.t Array4.t) * to_check) = {
+  proc __mul4_a24_rs (fs:W64.t Array4.t) : ((W64.t Array4.t) * trace) = {
     var aux_1:bool;
     var aux_0:W64.t;
     var aux:W64.t;
@@ -32,26 +32,16 @@ module M = {
     var  _2:bool;
     var  _3:bool;
     var  _4:bool;
-    var assume___mul4_a24_rs:bool;
-    var assert___mul4_a24_rs:bool;
-    var assume_proof___mul4_a24_rs:bool;
-    var assert_proof___mul4_a24_rs:bool;
-    assume___mul4_a24_rs <- true;
-    assert___mul4_a24_rs <- true;
-    assume_proof___mul4_a24_rs <- true;
-    assert_proof___mul4_a24_rs <- assert___mul4_a24_rs;
+    var old_fs:W64.t Array4.t;
+    var trace___mul4_a24_rs:trace;
+    old_fs <- fs;
+    trace___mul4_a24_rs <- [];
     h <- witness;
     c <- (W64.of_int 121665);
-    assert_proof___mul4_a24_rs <-
-    (assert_proof___mul4_a24_rs /\
-    ((assert___mul4_a24_rs /\ assume___mul4_a24_rs) =>
-    (c = (W64.of_int 121665))));
-    assert___mul4_a24_rs <-
-    (assert___mul4_a24_rs /\ (c = (W64.of_int 121665)));
-    assume_proof___mul4_a24_rs <-
-    (assume_proof___mul4_a24_rs /\
-    ((assert___mul4_a24_rs /\ assume___mul4_a24_rs) => ((u64i c) = 121665)));
-    assume___mul4_a24_rs <- (assume___mul4_a24_rs /\ ((u64i c) = 121665));
+    trace___mul4_a24_rs <-
+    (trace___mul4_a24_rs ++ [(Assert, (c = (W64.of_int 121665)))]);
+    trace___mul4_a24_rs <-
+    (trace___mul4_a24_rs ++ [(Assume, ((u64i c) = 121665))]);
     (aux_0, aux) <- (MULX_64 c fs.[0]);
     h.[1] <- aux_0;
     h.[0] <- aux;
@@ -73,14 +63,9 @@ module M = {
     h.[3] <- aux_0;
     (cf, r0) <- (adc_64 r0 (W64.of_int 0) cf);
     ( _0,  _1,  _2,  _3,  _4, r0) <- (IMULri_64 r0 (W64.of_int 38));
-    assert_proof___mul4_a24_rs <-
-    (assert_proof___mul4_a24_rs /\
-    ((assert___mul4_a24_rs /\ assume___mul4_a24_rs) => (! cf)));
-    assert___mul4_a24_rs <- (assert___mul4_a24_rs /\ (! cf));
-    assume_proof___mul4_a24_rs <-
-    (assume_proof___mul4_a24_rs /\
-    ((assert___mul4_a24_rs /\ assume___mul4_a24_rs) => ((b2i cf) = 0)));
-    assume___mul4_a24_rs <- (assume___mul4_a24_rs /\ ((b2i cf) = 0));
+    trace___mul4_a24_rs <- (trace___mul4_a24_rs ++ [(Assert, (! cf))]);
+    trace___mul4_a24_rs <-
+    (trace___mul4_a24_rs ++ [(Assume, ((b2i cf) = 0))]);
     (aux_1, aux_0) <- (adc_64 h.[0] r0 false);
     cf <- aux_1;
     h.[0] <- aux_0;
@@ -95,109 +80,105 @@ module M = {
     h.[3] <- aux_0;
     carryo <- cf;
     (cf, c) <- (sbb_64 c c cf);
-    assert_proof___mul4_a24_rs <-
-    (assert_proof___mul4_a24_rs /\
-    ((assert___mul4_a24_rs /\ assume___mul4_a24_rs) => (cf = carryo)));
-    assert___mul4_a24_rs <- (assert___mul4_a24_rs /\ (cf = carryo));
-    assume_proof___mul4_a24_rs <-
-    (assume_proof___mul4_a24_rs /\
-    ((assert___mul4_a24_rs /\ assume___mul4_a24_rs) =>
-    ((b2i cf) = (b2i carryo))));
-    assume___mul4_a24_rs <-
-    (assume___mul4_a24_rs /\ ((b2i cf) = (b2i carryo)));
+    trace___mul4_a24_rs <-
+    (trace___mul4_a24_rs ++ [(Assert, (cf = carryo))]);
+    trace___mul4_a24_rs <-
+    (trace___mul4_a24_rs ++ [(Assume, ((b2i cf) = (b2i carryo)))]);
     c <- (c `&` (W64.of_int 38));
-    assert_proof___mul4_a24_rs <-
-    (assert_proof___mul4_a24_rs /\
-    ((assert___mul4_a24_rs /\ assume___mul4_a24_rs) =>
-    (((! cf) /\ (c = (W64.of_int 0))) \/ (cf /\ (c = (W64.of_int 38))))));
-    assert___mul4_a24_rs <-
-    (assert___mul4_a24_rs /\
-    (((! cf) /\ (c = (W64.of_int 0))) \/ (cf /\ (c = (W64.of_int 38)))));
-    assume_proof___mul4_a24_rs <-
-    (assume_proof___mul4_a24_rs /\
-    ((assert___mul4_a24_rs /\ assume___mul4_a24_rs) =>
-    ((u64i c) = ((b2i cf) * 38))));
-    assume___mul4_a24_rs <-
-    (assume___mul4_a24_rs /\ ((u64i c) = ((b2i cf) * 38)));
+    trace___mul4_a24_rs <-
+    (trace___mul4_a24_rs ++
+    [(Assert,
+     (((! cf) /\ (c = (W64.of_int 0))) \/ (cf /\ (c = (W64.of_int 38)))))]);
+    trace___mul4_a24_rs <-
+    (trace___mul4_a24_rs ++ [(Assume, ((u64i c) = ((b2i cf) * 38)))]);
     (aux_1, aux_0) <- (adc_64 h.[0] c false);
     cf <- aux_1;
     h.[0] <- aux_0;
-    assert_proof___mul4_a24_rs <-
-    (assert_proof___mul4_a24_rs /\
-    ((assert___mul4_a24_rs /\ assume___mul4_a24_rs) => (! cf)));
-    assert___mul4_a24_rs <- (assert___mul4_a24_rs /\ (! cf));
-    assume_proof___mul4_a24_rs <-
-    (assume_proof___mul4_a24_rs /\
-    ((assert___mul4_a24_rs /\ assume___mul4_a24_rs) => ((b2i cf) = 0)));
-    assume___mul4_a24_rs <- (assume___mul4_a24_rs /\ ((b2i cf) = 0));
-    return (h,
-           (assume___mul4_a24_rs, assert___mul4_a24_rs,
-           assume_proof___mul4_a24_rs, assert_proof___mul4_a24_rs));
+    trace___mul4_a24_rs <- (trace___mul4_a24_rs ++ [(Assert, (! cf))]);
+    trace___mul4_a24_rs <-
+    (trace___mul4_a24_rs ++ [(Assume, ((b2i cf) = 0))]);
+    trace___mul4_a24_rs <-
+    (trace___mul4_a24_rs ++
+    [(Assert,
+     (eqmod
+     (foldr (fun x => (fun (acc:int) => (x + acc))) 0
+     (map (fun ii => ((pow 2 (64 * ii)) * (u64i h.[ii]))) (iota_ 0 4)))
+     ((foldr (fun x => (fun (acc:int) => (x + acc))) 0
+      (map (fun ii => ((pow 2 (64 * ii)) * (u64i old_fs.[ii]))) (iota_ 0 4))) *
+     121665) (single ((pow 2 255) - 19))))]);
+    return (h, trace___mul4_a24_rs);
   }
 }.
 
-(* All assume are valid. *)
+(* The post is in the trace. *)
 
-lemma __mul4_a24_rs_assume  :
-      hoare [M.__mul4_a24_rs : true ==> (assume_proof_ res)].
-proof.
-    proc. 
-    seq 32 : (assume_proof__ (assume___mul4_a24_rs, assert___mul4_a24_rs, assume_proof___mul4_a24_rs, assert_proof___mul4_a24_rs)). auto => />. 
-    seq 18 : (assume_proof__ (assume___mul4_a24_rs, assert___mul4_a24_rs, assume_proof___mul4_a24_rs, assert_proof___mul4_a24_rs)). auto => />.
-    auto => />. move => &hr H H0 H1 H2.
-    smt(@W64 @JUtils).
-qed.
-
-(* Soundness of assert/assume. *)
-
-lemma __mul4_a24_rs_assert_assume_sound  :
-      hoare [M.__mul4_a24_rs : true ==> (soundness_ res)].
-proof.
-    proc.
-    seq 10 : (soundness__ (assume___mul4_a24_rs, assert___mul4_a24_rs, assume_proof___mul4_a24_rs, assert_proof___mul4_a24_rs)). auto => />. 
-    seq 25 : (soundness__ (assume___mul4_a24_rs, assert___mul4_a24_rs, assume_proof___mul4_a24_rs, assert_proof___mul4_a24_rs)). auto => />. smt().
-    seq 23 : (soundness__ (assume___mul4_a24_rs, assert___mul4_a24_rs, assume_proof___mul4_a24_rs, assert_proof___mul4_a24_rs)). auto => />. smt().
-    auto => />. smt(). 
-qed.
-
-(* Lemmas proved by cryptoline. *)
-
-axiom __mul4_a24_rs_assert _fs :
+lemma __mul4_a24_rs_valid_post _fs :
       hoare [M.__mul4_a24_rs :
-      ((_fs = fs) /\ true) ==>
-      (_assert_spec res
+      (_fs = fs) ==>
+      ((valid (trace res)) =>
       (eqmod
-      (foldr (fun x => (fun (acc: int) => (x + acc))) 0
+      (foldr (fun x => (fun (acc:int) => (x + acc))) 0
       (map (fun ii => ((pow 2 (64 * ii)) * (u64i res.`1.[ii]))) (iota_ 0 4)))
-      ((foldr (fun x => (fun (acc: int) => (x + acc))) 0
+      ((foldr (fun x => (fun (acc:int) => (x + acc))) 0
        (map (fun ii => ((pow 2 (64 * ii)) * (u64i _fs.[ii]))) (iota_ 0 4))) *
       121665) (single ((pow 2 255) - 19))))].
+proof.
+proc .
+wp -1 => /=.
+conseq (:  _ ==> (_fs = old_fs)).
+move => ? _ /> 2?.
+rewrite /trace /= valid_cat /valid //=.
+seq 1 : ((_fs = old_fs)).
+by auto .
+by conseq  />.
+qed .
+
+(* The post is in the trace and all assumes are valid. *)
+
+lemma __mul4_a24_rs_assume_ _fs :
+      hoare [M.__mul4_a24_rs :
+      (_fs = fs) ==> (true => (validk Assume (trace res)))].
+proof.
+    proc. auto => />. smt(@Zp_25519 @JUtils @W64 @Jcheck).
+qed.
+
+lemma __mul4_a24_rs_assume _fs :
+      hoare [M.__mul4_a24_rs :
+      (_fs = fs) ==>
+      (((valid (trace res)) =>
+       (eqmod
+       (foldr (fun x => (fun (acc:int) => (x + acc))) 0
+       (map (fun ii => ((pow 2 (64 * ii)) * (u64i res.`1.[ii]))) (iota_ 0 4))
+       )
+       ((foldr (fun x => (fun (acc:int) => (x + acc))) 0
+        (map (fun ii => ((pow 2 (64 * ii)) * (u64i _fs.[ii]))) (iota_ 0 4))) *
+       121665) (single ((pow 2 255) - 19)))) /\
+      (true => (validk Assume (trace res))))].
+proof.
+conseq (__mul4_a24_rs_assume_ _fs) (__mul4_a24_rs_valid_post _fs) => />.
+qed .
+
+(* All assert are valid. *)
+
+lemma __mul4_a24_rs_assert _fs :
+      hoare [M.__mul4_a24_rs :
+      ((_fs = fs) /\ true) ==> (validk Assert (trace res))].
+proof.
+admitted (* Proven by Cryptoline *).
 
 (* Final specification for the functions. *)
 
-lemma __mul4_a24_rs_spec  :
-      forall _fs,
+lemma __mul4_a24_rs_spec _fs :
       hoare [M.__mul4_a24_rs :
       ((_fs = fs) /\ true) ==>
       (eqmod
-      (foldr (fun x => (fun (acc: int) => (x + acc))) 0
+      (foldr (fun x => (fun (acc:int) => (x + acc))) 0
       (map (fun ii => ((pow 2 (64 * ii)) * (u64i res.`1.[ii]))) (iota_ 0 4)))
-      ((foldr (fun x => (fun (acc: int) => (x + acc))) 0
+      ((foldr (fun x => (fun (acc:int) => (x + acc))) 0
        (map (fun ii => ((pow 2 (64 * ii)) * (u64i _fs.[ii]))) (iota_ 0 4))) *
       121665) (single ((pow 2 255) - 19)))].
 proof.
-move => _fs.
-have h  :
-     hoare [M.__mul4_a24_rs :
-     ((_fs = fs) /\ true) ==>
-     (_spec_soundness res
-     (eqmod
-     (foldr (fun x => (fun (acc: int) => (x + acc))) 0
-     (map (fun ii => ((pow 2 (64 * ii)) * (u64i res.`1.[ii]))) (iota_ 0 4)))
-     ((foldr (fun x => (fun (acc: int) => (x + acc))) 0
-      (map (fun ii => ((pow 2 (64 * ii)) * (u64i _fs.[ii]))) (iota_ 0 4))) *
-     121665) (single ((pow 2 255) - 19))))].
-by conseq __mul4_a24_rs_assume (__mul4_a24_rs_assert _fs).
-conseq h __mul4_a24_rs_assert_assume_sound => // ; smt ().
+conseq (__mul4_a24_rs_assume _fs) (__mul4_a24_rs_assert _fs) => />.
+smt (all_validk_valid).
 qed .
 
