proof/crypto_scalarmult/curve25519/amd64/cryptoline_extraction/Mul4_a24RefExtracted.ec
@@ -4,23 +4,20 @@ from Jasmin require import JModel_x86.
 
 import SLH64.
 
-require import Jcheck.
+from Jasmin require import Jcheck.
 
 require import Array4.
 
 require import WArray32.
 
-
-
-require import Jcheck Zp_limbs Zp_25519 CommonCryptoline.
+require import Zp_limbs Zp_25519 CommonCryptoline.
 import Zp_25519 Zp Zp_limbs EClib.
 
-
 module M = {
-  var tmp__check : to_check
+  var tmp__trace : trace
   var tmp__data___mul4_a24_rs : (W64.t Array4.t)
   var tmp____mul4_a24_rs : W64.t Array4.t
-  proc __mul4_a24_rs (xa:W64.t Array4.t) : ((W64.t Array4.t) * to_check) = {
+  proc __mul4_a24_rs (xa:W64.t Array4.t) : ((W64.t Array4.t) * trace) = {
     var aux:bool;
     var aux_0:W64.t;
     var r:W64.t Array4.t;
@@ -33,26 +30,16 @@ module M = {
     var t4:W64.t;
     var cf:bool;
     var dc:W64.t;
-    var assume___mul4_a24_rs:bool;
-    var assert___mul4_a24_rs:bool;
-    var assume_proof___mul4_a24_rs:bool;
-    var assert_proof___mul4_a24_rs:bool;
-    assume___mul4_a24_rs <- true;
-    assert___mul4_a24_rs <- true;
-    assume_proof___mul4_a24_rs <- true;
-    assert_proof___mul4_a24_rs <- assert___mul4_a24_rs;
+    var old_xa:W64.t Array4.t;
+    var trace___mul4_a24_rs:trace;
+    old_xa <- xa;
+    trace___mul4_a24_rs <- [];
     r <- witness;
     c <- (W64.of_int 121665);
-    assert_proof___mul4_a24_rs <-
-    (assert_proof___mul4_a24_rs /\
-    ((assert___mul4_a24_rs /\ assume___mul4_a24_rs) =>
-    (c = (W64.of_int 121665))));
-    assert___mul4_a24_rs <-
-    (assert___mul4_a24_rs /\ (c = (W64.of_int 121665)));
-    assume_proof___mul4_a24_rs <-
-    (assume_proof___mul4_a24_rs /\
-    ((assert___mul4_a24_rs /\ assume___mul4_a24_rs) => ((u64i c) = 121665)));
-    assume___mul4_a24_rs <- (assume___mul4_a24_rs /\ ((u64i c) = 121665));
+    trace___mul4_a24_rs <-
+    (trace___mul4_a24_rs ++ [(Assert, (c = (W64.of_int 121665)))]);
+    trace___mul4_a24_rs <-
+    (trace___mul4_a24_rs ++ [(Assume, ((u64i c) = 121665))]);
     rax <- xa.[0];
     (rdx, rax) <- (mulu_64 rax c);
     r.[0] <- rax;
@@ -79,23 +66,14 @@ module M = {
     cf <- aux;
     r.[3] <- aux_0;
     (cf, t4) <- (adc_64 t4 (W64.of_int 0) cf);
-    assert_proof___mul4_a24_rs <-
-    (assert_proof___mul4_a24_rs /\
-    ((assert___mul4_a24_rs /\ assume___mul4_a24_rs) => (! cf)));
-    assert___mul4_a24_rs <- (assert___mul4_a24_rs /\ (! cf));
-    assume_proof___mul4_a24_rs <-
-    (assume_proof___mul4_a24_rs /\
-    ((assert___mul4_a24_rs /\ assume___mul4_a24_rs) => ((b2i cf) = 0)));
-    assume___mul4_a24_rs <- (assume___mul4_a24_rs /\ ((b2i cf) = 0));
+    trace___mul4_a24_rs <- (trace___mul4_a24_rs ++ [(Assert, (! cf))]);
+    trace___mul4_a24_rs <-
+    (trace___mul4_a24_rs ++ [(Assume, ((b2i cf) = 0))]);
     (dc, t4) <- (mulu_64 t4 (W64.of_int 38));
-    assert_proof___mul4_a24_rs <-
-    (assert_proof___mul4_a24_rs /\
-    ((assert___mul4_a24_rs /\ assume___mul4_a24_rs) => (dc = (W64.of_int 0))));
-    assert___mul4_a24_rs <- (assert___mul4_a24_rs /\ (dc = (W64.of_int 0)));
-    assume_proof___mul4_a24_rs <-
-    (assume_proof___mul4_a24_rs /\
-    ((assert___mul4_a24_rs /\ assume___mul4_a24_rs) => (dc = (W64.of_int 0))));
-    assume___mul4_a24_rs <- (assume___mul4_a24_rs /\ (dc = (W64.of_int 0)));
+    trace___mul4_a24_rs <-
+    (trace___mul4_a24_rs ++ [(Assert, (dc = (W64.of_int 0)))]);
+    trace___mul4_a24_rs <-
+    (trace___mul4_a24_rs ++ [(Assume, (dc = (W64.of_int 0)))]);
     (aux, aux_0) <- (adc_64 r.[0] t4 false);
     cf <- aux;
     r.[0] <- aux_0;
@@ -114,74 +92,91 @@ module M = {
     (aux, aux_0) <- (adc_64 r.[0] t1 false);
     cf <- aux;
     r.[0] <- aux_0;
-    assert_proof___mul4_a24_rs <-
-    (assert_proof___mul4_a24_rs /\
-    ((assert___mul4_a24_rs /\ assume___mul4_a24_rs) => (! cf)));
-    assert___mul4_a24_rs <- (assert___mul4_a24_rs /\ (! cf));
-    assume_proof___mul4_a24_rs <-
-    (assume_proof___mul4_a24_rs /\
-    ((assert___mul4_a24_rs /\ assume___mul4_a24_rs) => ((b2i cf) = 0)));
-    assume___mul4_a24_rs <- (assume___mul4_a24_rs /\ ((b2i cf) = 0));
-    return (r,
-           (assume___mul4_a24_rs, assert___mul4_a24_rs,
-           assume_proof___mul4_a24_rs, assert_proof___mul4_a24_rs));
+    trace___mul4_a24_rs <- (trace___mul4_a24_rs ++ [(Assert, (! cf))]);
+    trace___mul4_a24_rs <-
+    (trace___mul4_a24_rs ++ [(Assume, ((b2i cf) = 0))]);
+    trace___mul4_a24_rs <-
+    (trace___mul4_a24_rs ++
+    [(Assert,
+     (eqmod
+     (foldr (fun x => (fun (acc:int) => (x + acc))) 0
+     (map (fun ii => ((pow 2 (64 * ii)) * (u64i r.[ii]))) (iota_ 0 4)))
+     ((foldr (fun x => (fun (acc:int) => (x + acc))) 0
+      (map (fun ii => ((pow 2 (64 * ii)) * (u64i old_xa.[ii]))) (iota_ 0 4))) *
+     121665) (single ((pow 2 255) - 19))))]);
+    return (r, trace___mul4_a24_rs);
   }
 }.
 
-(* All assume are valid. *)
+(* The post is in the trace. *)
 
-lemma __mul4_a24_rs_assume  :
-      hoare [M.__mul4_a24_rs : true ==> (assume_proof_ res)].
+lemma __mul4_a24_rs_valid_post _xa :
+      hoare [M.__mul4_a24_rs :
+      (_xa = xa) ==>
+      ((valid (trace res)) =>
+      (eqmod
+      (foldr (fun x => (fun (acc:int) => (x + acc))) 0
+      (map (fun ii => ((pow 2 (64 * ii)) * (u64i res.`1.[ii]))) (iota_ 0 4)))
+      ((foldr (fun x => (fun (acc:int) => (x + acc))) 0
+       (map (fun ii => ((pow 2 (64 * ii)) * (u64i _xa.[ii]))) (iota_ 0 4))) *
+      121665) (single ((pow 2 255) - 19))))].
+proof.
+proc .
+wp -1 => /=.
+conseq (:  _ ==> (_xa = old_xa)).
+move => ? _ /> 2?.
+rewrite /trace /= valid_cat /valid //=.
+seq 1 : ((_xa = old_xa)).
+by auto .
+by conseq  />.
+qed .
+
+(* The post is in the trace and all assumes are valid. *)
+
+lemma __mul4_a24_rs_assume_ _xa :
+      hoare [M.__mul4_a24_rs :
+      (_xa = xa) ==> (true => (validk Assume (trace res)))].
 proof.
     proc. auto => />.
 qed.
 
-(* Soundness of assert/assume. *)
-
-lemma __mul4_a24_rs_assert_assume_sound  :
-      hoare [M.__mul4_a24_rs : true ==> (soundness_ res)].
-proof.
-    proc. auto => />. smt(@W64 @Zp_25519).
-qed.
-
-(* Lemmas proved by cryptoline. *)
-
-axiom __mul4_a24_rs_assert _xa :
+lemma __mul4_a24_rs_assume _xa :
       hoare [M.__mul4_a24_rs :
-      ((_xa = xa) /\ true) ==>
-      (_assert_spec res
-      (eqmod
-      (foldr (fun x => (fun (acc: int) => (x + acc))) 0
-      (map (fun ii => ((pow 2 (64 * ii)) * (u64i res.`1.[ii]))) (iota_ 0 4)))
-      ((foldr (fun x => (fun (acc: int) => (x + acc))) 0
-       (map (fun ii => ((pow 2 (64 * ii)) * (u64i _xa.[ii]))) (iota_ 0 4))) *
-      121665) (single ((pow 2 255) - 19))))].
+      (_xa = xa) ==>
+      (((valid (trace res)) =>
+       (eqmod
+       (foldr (fun x => (fun (acc:int) => (x + acc))) 0
+       (map (fun ii => ((pow 2 (64 * ii)) * (u64i res.`1.[ii]))) (iota_ 0 4))
+       )
+       ((foldr (fun x => (fun (acc:int) => (x + acc))) 0
+        (map (fun ii => ((pow 2 (64 * ii)) * (u64i _xa.[ii]))) (iota_ 0 4))) *
+       121665) (single ((pow 2 255) - 19)))) /\
+      (true => (validk Assume (trace res))))].
+proof.
+conseq (__mul4_a24_rs_assume_ _xa) (__mul4_a24_rs_valid_post _xa) => />.
+qed .
+
+(* All assert are valid. *)
+
+lemma __mul4_a24_rs_assert _xa :
+      hoare [M.__mul4_a24_rs :
+      ((_xa = xa) /\ true) ==> (validk Assert (trace res))].
+proof.
+admitted (* Proven by Cryptoline *).
 
 (* Final specification for the functions. *)
 
-lemma __mul4_a24_rs_spec  :
-      forall _xa,
+lemma __mul4_a24_rs_spec _xa :
       hoare [M.__mul4_a24_rs :
       ((_xa = xa) /\ true) ==>
       (eqmod
-      (foldr (fun x => (fun (acc: int) => (x + acc))) 0
+      (foldr (fun x => (fun (acc:int) => (x + acc))) 0
       (map (fun ii => ((pow 2 (64 * ii)) * (u64i res.`1.[ii]))) (iota_ 0 4)))
-      ((foldr (fun x => (fun (acc: int) => (x + acc))) 0
+      ((foldr (fun x => (fun (acc:int) => (x + acc))) 0
        (map (fun ii => ((pow 2 (64 * ii)) * (u64i _xa.[ii]))) (iota_ 0 4))) *
       121665) (single ((pow 2 255) - 19)))].
 proof.
-move => _xa.
-have h  :
-     hoare [M.__mul4_a24_rs :
-     ((_xa = xa) /\ true) ==>
-     (_spec_soundness res
-     (eqmod
-     (foldr (fun x => (fun (acc: int) => (x + acc))) 0
-     (map (fun ii => ((pow 2 (64 * ii)) * (u64i res.`1.[ii]))) (iota_ 0 4)))
-     ((foldr (fun x => (fun (acc: int) => (x + acc))) 0
-      (map (fun ii => ((pow 2 (64 * ii)) * (u64i _xa.[ii]))) (iota_ 0 4))) *
-     121665) (single ((pow 2 255) - 19))))].
-by conseq __mul4_a24_rs_assume (__mul4_a24_rs_assert _xa).
-conseq h __mul4_a24_rs_assert_assume_sound => // ; smt ().
+conseq (__mul4_a24_rs_assume _xa) (__mul4_a24_rs_assert _xa) => />.
+smt (all_validk_valid).
 qed .
 
