proof/crypto_scalarmult/curve25519/amd64/cryptoline_extraction/Sqr4RefExtracted.ec
@@ -4,44 +4,46 @@ from Jasmin require import JModel_x86.
 
 import SLH64.
 
-require import Jcheck.
+from Jasmin require import Jcheck.
 
 require import Array4 Array5 Array8.
 
 require import WArray32 WArray40 WArray64.
 
-require import Jcheck Zp_limbs Zp_25519 CommonCryptoline.
+require import Zp_limbs Zp_25519 CommonCryptoline.
 import Zp_25519 Zp Zp_limbs EClib.
 
 module M = {
-  var tmp__check : to_check
+  var tmp__trace : trace
   var tmp__data___reduce4 : (W64.t Array4.t)
   var tmp____reduce4 : W64.t Array4.t
   var tmp__data___sqr4_rs : (W64.t Array4.t)
   var tmp____sqr4_rs : W64.t Array4.t
-  proc __reduce4 (z:W64.t Array8.t) : ((W64.t Array4.t) * to_check) = {
+  proc __reduce4 (z:W64.t Array8.t) : ((W64.t Array4.t) * trace) = {
     var aux:bool;
     var aux_1:int;
     var aux_0:W64.t;
     var r:W64.t Array4.t;
+    var cf:bool;
     var r38:W64.t;
     var rax:W64.t;
     var h:W64.t;
     var l:W64.t;
-    var cf:bool;
     var z8:W64.t;
     var i:int;
     var dc:W64.t;
     var r0:W64.t;
-    var assume___reduce4:bool;
-    var assert___reduce4:bool;
-    var assume_proof___reduce4:bool;
-    var assert_proof___reduce4:bool;
-    assume___reduce4 <- true;
-    assert___reduce4 <- true;
-    assume_proof___reduce4 <- true;
-    assert_proof___reduce4 <- assert___reduce4;
+    var  _0:bool;
+    var  _1:bool;
+    var  _2:bool;
+    var  _3:bool;
+    var  _4:W64.t;
+    var old_z:W64.t Array8.t;
+    var trace___reduce4:trace;
+    old_z <- z;
+    trace___reduce4 <- [];
     r <- witness;
+    ( _0, cf,  _1,  _2,  _3,  _4) <- (set0_64);
     r38 <- (W64.of_int 38);
     rax <- z.[4];
     (h, l) <- (mulu_64 rax r38);
@@ -57,14 +59,8 @@ module M = {
     (aux, aux_0) <- (adc_64 r.[2] h cf);
     cf <- aux;
     r.[2] <- aux_0;
-    assert_proof___reduce4 <-
-    (assert_proof___reduce4 /\
-    ((assert___reduce4 /\ assume___reduce4) => (! cf)));
-    assert___reduce4 <- (assert___reduce4 /\ (! cf));
-    assume_proof___reduce4 <-
-    (assume_proof___reduce4 /\
-    ((assert___reduce4 /\ assume___reduce4) => ((b2i cf) = 0)));
-    assume___reduce4 <- (assume___reduce4 /\ ((b2i cf) = 0));
+    trace___reduce4 <- (trace___reduce4 ++ [(Assert, (! cf))]);
+    trace___reduce4 <- (trace___reduce4 ++ [(Assume, ((b2i cf) = 0))]);
     (h, l) <- (mulu_64 rax r38);
     (aux, aux_0) <- (adc_64 r.[2] l false);
     cf <- aux;
@@ -74,28 +70,16 @@ module M = {
     (aux, aux_0) <- (adc_64 r.[3] h cf);
     cf <- aux;
     r.[3] <- aux_0;
-    assert_proof___reduce4 <-
-    (assert_proof___reduce4 /\
-    ((assert___reduce4 /\ assume___reduce4) => (! cf)));
-    assert___reduce4 <- (assert___reduce4 /\ (! cf));
-    assume_proof___reduce4 <-
-    (assume_proof___reduce4 /\
-    ((assert___reduce4 /\ assume___reduce4) => ((b2i cf) = 0)));
-    assume___reduce4 <- (assume___reduce4 /\ ((b2i cf) = 0));
+    trace___reduce4 <- (trace___reduce4 ++ [(Assert, (! cf))]);
+    trace___reduce4 <- (trace___reduce4 ++ [(Assume, ((b2i cf) = 0))]);
     (h, l) <- (mulu_64 rax r38);
     (aux, aux_0) <- (adc_64 r.[3] l false);
     cf <- aux;
     r.[3] <- aux_0;
     z8 <- (MOV_64 (W64.of_int 0));
     (cf, z8) <- (adc_64 z8 h cf);
-    assert_proof___reduce4 <-
-    (assert_proof___reduce4 /\
-    ((assert___reduce4 /\ assume___reduce4) => (! cf)));
-    assert___reduce4 <- (assert___reduce4 /\ (! cf));
-    assume_proof___reduce4 <-
-    (assume_proof___reduce4 /\
-    ((assert___reduce4 /\ assume___reduce4) => ((b2i cf) = 0)));
-    assume___reduce4 <- (assume___reduce4 /\ ((b2i cf) = 0));
+    trace___reduce4 <- (trace___reduce4 ++ [(Assert, (! cf))]);
+    trace___reduce4 <- (trace___reduce4 ++ [(Assume, ((b2i cf) = 0))]);
     (aux, aux_0) <- (adc_64 r.[0] z.[0] false);
     cf <- aux;
     r.[0] <- aux_0;
@@ -107,23 +91,13 @@ module M = {
       i <- (i + 1);
     }
     (cf, z8) <- (adc_64 z8 (W64.of_int 0) cf);
-    assert_proof___reduce4 <-
-    (assert_proof___reduce4 /\
-    ((assert___reduce4 /\ assume___reduce4) => (! cf)));
-    assert___reduce4 <- (assert___reduce4 /\ (! cf));
-    assume_proof___reduce4 <-
-    (assume_proof___reduce4 /\
-    ((assert___reduce4 /\ assume___reduce4) => ((b2i cf) = 0)));
-    assume___reduce4 <- (assume___reduce4 /\ ((b2i cf) = 0));
+    trace___reduce4 <- (trace___reduce4 ++ [(Assert, (! cf))]);
+    trace___reduce4 <- (trace___reduce4 ++ [(Assume, ((b2i cf) = 0))]);
     (dc, z8) <- (mulu_64 z8 (W64.of_int 38));
-    assert_proof___reduce4 <-
-    (assert_proof___reduce4 /\
-    ((assert___reduce4 /\ assume___reduce4) => (dc = (W64.of_int 0))));
-    assert___reduce4 <- (assert___reduce4 /\ (dc = (W64.of_int 0)));
-    assume_proof___reduce4 <-
-    (assume_proof___reduce4 /\
-    ((assert___reduce4 /\ assume___reduce4) => (dc = (W64.of_int 0))));
-    assume___reduce4 <- (assume___reduce4 /\ (dc = (W64.of_int 0)));
+    trace___reduce4 <-
+    (trace___reduce4 ++ [(Assert, (dc = (W64.of_int 0)))]);
+    trace___reduce4 <-
+    (trace___reduce4 ++ [(Assume, (dc = (W64.of_int 0)))]);
     r0 <- (MOV_64 (W64.of_int 0));
     (aux, aux_0) <- (adc_64 r.[0] z8 false);
     cf <- aux;
@@ -136,39 +110,30 @@ module M = {
       i <- (i + 1);
     }
     (cf, r0) <- (adc_64 r0 r0 cf);
-    assert_proof___reduce4 <-
-    (assert_proof___reduce4 /\
-    ((assert___reduce4 /\ assume___reduce4) => (! cf)));
-    assert___reduce4 <- (assert___reduce4 /\ (! cf));
-    assume_proof___reduce4 <-
-    (assume_proof___reduce4 /\
-    ((assert___reduce4 /\ assume___reduce4) => ((b2i cf) = 0)));
-    assume___reduce4 <- (assume___reduce4 /\ ((b2i cf) = 0));
+    trace___reduce4 <- (trace___reduce4 ++ [(Assert, (! cf))]);
+    trace___reduce4 <- (trace___reduce4 ++ [(Assume, ((b2i cf) = 0))]);
     (dc, r0) <- (mulu_64 r0 (W64.of_int 38));
-    assert_proof___reduce4 <-
-    (assert_proof___reduce4 /\
-    ((assert___reduce4 /\ assume___reduce4) => (dc = (W64.of_int 0))));
-    assert___reduce4 <- (assert___reduce4 /\ (dc = (W64.of_int 0)));
-    assume_proof___reduce4 <-
-    (assume_proof___reduce4 /\
-    ((assert___reduce4 /\ assume___reduce4) => (dc = (W64.of_int 0))));
-    assume___reduce4 <- (assume___reduce4 /\ (dc = (W64.of_int 0)));
+    trace___reduce4 <-
+    (trace___reduce4 ++ [(Assert, (dc = (W64.of_int 0)))]);
+    trace___reduce4 <-
+    (trace___reduce4 ++ [(Assume, (dc = (W64.of_int 0)))]);
     (aux, aux_0) <- (adc_64 r.[0] r0 false);
     cf <- aux;
     r.[0] <- aux_0;
-    assert_proof___reduce4 <-
-    (assert_proof___reduce4 /\
-    ((assert___reduce4 /\ assume___reduce4) => (! cf)));
-    assert___reduce4 <- (assert___reduce4 /\ (! cf));
-    assume_proof___reduce4 <-
-    (assume_proof___reduce4 /\
-    ((assert___reduce4 /\ assume___reduce4) => ((b2i cf) = 0)));
-    assume___reduce4 <- (assume___reduce4 /\ ((b2i cf) = 0));
-    return (r,
-           (assume___reduce4, assert___reduce4, assume_proof___reduce4,
-           assert_proof___reduce4));
+    trace___reduce4 <- (trace___reduce4 ++ [(Assert, (! cf))]);
+    trace___reduce4 <- (trace___reduce4 ++ [(Assume, ((b2i cf) = 0))]);
+    trace___reduce4 <-
+    (trace___reduce4 ++
+    [(Assert,
+     (eqmod
+     (foldr (fun x => (fun (acc:int) => (x + acc))) 0
+     (map (fun ii => ((pow 2 (64 * ii)) * (u64i r.[ii]))) (iota_ 0 4)))
+     (foldr (fun x => (fun (acc:int) => (x + acc))) 0
+     (map (fun ii => ((pow 2 (64 * ii)) * (u64i old_z.[ii]))) (iota_ 0 8)))
+     (single ((pow 2 255) - 19))))]);
+    return (r, trace___reduce4);
   }
-  proc __sqr4_rs (xa:W64.t Array4.t) : ((W64.t Array4.t) * to_check) = {
+  proc __sqr4_rs (xa:W64.t Array4.t) : ((W64.t Array4.t) * trace) = {
     var aux:bool;
     var aux_0:W64.t;
     var r:W64.t Array4.t;
@@ -178,14 +143,10 @@ module M = {
     var rdx:W64.t;
     var cf:bool;
     var t:W64.t Array5.t;
-    var assume___sqr4_rs:bool;
-    var assert___sqr4_rs:bool;
-    var assume_proof___sqr4_rs:bool;
-    var assert_proof___sqr4_rs:bool;
-    assume___sqr4_rs <- true;
-    assert___sqr4_rs <- true;
-    assume_proof___sqr4_rs <- true;
-    assert_proof___sqr4_rs <- assert___sqr4_rs;
+    var old_xa:W64.t Array4.t;
+    var trace___sqr4_rs:trace;
+    old_xa <- xa;
+    trace___sqr4_rs <- [];
     r <- witness;
     t <- witness;
     z <- witness;
@@ -214,14 +175,8 @@ module M = {
     (aux, aux_0) <- (adc_64 z.[4] zero cf);
     cf <- aux;
     z.[4] <- aux_0;
-    assert_proof___sqr4_rs <-
-    (assert_proof___sqr4_rs /\
-    ((assert___sqr4_rs /\ assume___sqr4_rs) => (! cf)));
-    assert___sqr4_rs <- (assert___sqr4_rs /\ (! cf));
-    assume_proof___sqr4_rs <-
-    (assume_proof___sqr4_rs /\
-    ((assert___sqr4_rs /\ assume___sqr4_rs) => ((b2i cf) = 0)));
-    assume___sqr4_rs <- (assume___sqr4_rs /\ ((b2i cf) = 0));
+    trace___sqr4_rs <- (trace___sqr4_rs ++ [(Assert, (! cf))]);
+    trace___sqr4_rs <- (trace___sqr4_rs ++ [(Assume, ((b2i cf) = 0))]);
     rax <- xa.[3];
     (rdx, rax) <- (mulu_64 rax xa.[1]);
     (aux, aux_0) <- (adc_64 z.[4] rax false);
@@ -233,14 +188,8 @@ module M = {
     (aux, aux_0) <- (adc_64 z.[6] zero cf);
     cf <- aux;
     z.[6] <- aux_0;
-    assert_proof___sqr4_rs <-
-    (assert_proof___sqr4_rs /\
-    ((assert___sqr4_rs /\ assume___sqr4_rs) => (! cf)));
-    assert___sqr4_rs <- (assert___sqr4_rs /\ (! cf));
-    assume_proof___sqr4_rs <-
-    (assume_proof___sqr4_rs /\
-    ((assert___sqr4_rs /\ assume___sqr4_rs) => ((b2i cf) = 0)));
-    assume___sqr4_rs <- (assume___sqr4_rs /\ ((b2i cf) = 0));
+    trace___sqr4_rs <- (trace___sqr4_rs ++ [(Assert, (! cf))]);
+    trace___sqr4_rs <- (trace___sqr4_rs ++ [(Assume, ((b2i cf) = 0))]);
     rax <- xa.[3];
     (rdx, rax) <- (mulu_64 rax xa.[0]);
     (aux, aux_0) <- (adc_64 z.[3] rax false);
@@ -258,14 +207,8 @@ module M = {
     (aux, aux_0) <- (adc_64 z.[7] zero cf);
     cf <- aux;
     z.[7] <- aux_0;
-    assert_proof___sqr4_rs <-
-    (assert_proof___sqr4_rs /\
-    ((assert___sqr4_rs /\ assume___sqr4_rs) => (! cf)));
-    assert___sqr4_rs <- (assert___sqr4_rs /\ (! cf));
-    assume_proof___sqr4_rs <-
-    (assume_proof___sqr4_rs /\
-    ((assert___sqr4_rs /\ assume___sqr4_rs) => ((b2i cf) = 0)));
-    assume___sqr4_rs <- (assume___sqr4_rs /\ ((b2i cf) = 0));
+    trace___sqr4_rs <- (trace___sqr4_rs ++ [(Assert, (! cf))]);
+    trace___sqr4_rs <- (trace___sqr4_rs ++ [(Assume, ((b2i cf) = 0))]);
     (aux, aux_0) <- (adc_64 z.[1] z.[1] false);
     cf <- aux;
     z.[1] <- aux_0;
@@ -287,14 +230,8 @@ module M = {
     (aux, aux_0) <- (adc_64 z.[7] z.[7] cf);
     cf <- aux;
     z.[7] <- aux_0;
-    assert_proof___sqr4_rs <-
-    (assert_proof___sqr4_rs /\
-    ((assert___sqr4_rs /\ assume___sqr4_rs) => (! cf)));
-    assert___sqr4_rs <- (assert___sqr4_rs /\ (! cf));
-    assume_proof___sqr4_rs <-
-    (assume_proof___sqr4_rs /\
-    ((assert___sqr4_rs /\ assume___sqr4_rs) => ((b2i cf) = 0)));
-    assume___sqr4_rs <- (assume___sqr4_rs /\ ((b2i cf) = 0));
+    trace___sqr4_rs <- (trace___sqr4_rs ++ [(Assert, (! cf))]);
+    trace___sqr4_rs <- (trace___sqr4_rs ++ [(Assume, ((b2i cf) = 0))]);
     rax <- xa.[0];
     (rdx, rax) <- (mulu_64 rax xa.[0]);
     z.[0] <- rax;
@@ -328,14 +265,8 @@ module M = {
     (aux, aux_0) <- (adc_64 z.[7] (W64.of_int 0) cf);
     cf <- aux;
     z.[7] <- aux_0;
-    assert_proof___sqr4_rs <-
-    (assert_proof___sqr4_rs /\
-    ((assert___sqr4_rs /\ assume___sqr4_rs) => (! cf)));
-    assert___sqr4_rs <- (assert___sqr4_rs /\ (! cf));
-    assume_proof___sqr4_rs <-
-    (assume_proof___sqr4_rs /\
-    ((assert___sqr4_rs /\ assume___sqr4_rs) => ((b2i cf) = 0)));
-    assume___sqr4_rs <- (assume___sqr4_rs /\ ((b2i cf) = 0));
+    trace___sqr4_rs <- (trace___sqr4_rs ++ [(Assert, (! cf))]);
+    trace___sqr4_rs <- (trace___sqr4_rs ++ [(Assume, ((b2i cf) = 0))]);
     rax <- xa.[3];
     (rdx, rax) <- (mulu_64 rax xa.[3]);
     (aux, aux_0) <- (adc_64 z.[6] rax false);
@@ -344,181 +275,185 @@ module M = {
     (aux, aux_0) <- (adc_64 z.[7] rdx cf);
     cf <- aux;
     z.[7] <- aux_0;
-    assert_proof___sqr4_rs <-
-    (assert_proof___sqr4_rs /\
-    ((assert___sqr4_rs /\ assume___sqr4_rs) => (! cf)));
-    assert___sqr4_rs <- (assert___sqr4_rs /\ (! cf));
-    assume_proof___sqr4_rs <-
-    (assume_proof___sqr4_rs /\
-    ((assert___sqr4_rs /\ assume___sqr4_rs) => ((b2i cf) = 0)));
-    assume___sqr4_rs <- (assume___sqr4_rs /\ ((b2i cf) = 0));
-    (tmp__data___reduce4, tmp__check) <@ __reduce4 (z);
+    trace___sqr4_rs <- (trace___sqr4_rs ++ [(Assert, (! cf))]);
+    trace___sqr4_rs <- (trace___sqr4_rs ++ [(Assume, ((b2i cf) = 0))]);
+    (tmp__data___reduce4, tmp__trace) <@ __reduce4 (z);
     tmp____reduce4 <- tmp__data___reduce4;
-    (assume___sqr4_rs, assert___sqr4_rs, assume_proof___sqr4_rs,
-    assert_proof___sqr4_rs) <-
-    (upd_call
-    (assume___sqr4_rs, assert___sqr4_rs, assume_proof___sqr4_rs,
-    assert_proof___sqr4_rs) tmp__check);
-    assert_proof___sqr4_rs <-
-    (assert_proof___sqr4_rs /\
-    ((assert___sqr4_rs /\ assume___sqr4_rs) =>
-    (eqmod
-    (foldr (fun x => (fun (acc: int) => (x + acc))) 0
-    (map (fun ii => ((pow 2 (64 * ii)) * (u64i tmp____reduce4.[ii])))
-    (iota_ 0 4)))
-    (foldr (fun x => (fun (acc: int) => (x + acc))) 0
-    (map (fun ii => ((pow 2 (64 * ii)) * (u64i z.[ii]))) (iota_ 0 8)))
-    (single ((pow 2 255) - 19)))));
-    assert___sqr4_rs <-
-    (assert___sqr4_rs /\
-    (eqmod
-    (foldr (fun x => (fun (acc: int) => (x + acc))) 0
-    (map (fun ii => ((pow 2 (64 * ii)) * (u64i tmp____reduce4.[ii])))
-    (iota_ 0 4)))
-    (foldr (fun x => (fun (acc: int) => (x + acc))) 0
-    (map (fun ii => ((pow 2 (64 * ii)) * (u64i z.[ii]))) (iota_ 0 8)))
-    (single ((pow 2 255) - 19))));
+    trace___sqr4_rs <- (trace___sqr4_rs ++ tmp__trace);
+    trace___sqr4_rs <-
+    (trace___sqr4_rs ++
+    [(Assume,
+     (eqmod
+     (foldr (fun x => (fun (acc:int) => (x + acc))) 0
+     (map (fun ii => ((pow 2 (64 * ii)) * (u64i tmp____reduce4.[ii])))
+     (iota_ 0 4)))
+     (foldr (fun x => (fun (acc:int) => (x + acc))) 0
+     (map (fun ii => ((pow 2 (64 * ii)) * (u64i z.[ii]))) (iota_ 0 8)))
+     (single ((pow 2 255) - 19))))]);
     r <- tmp____reduce4;
-    return (r,
-           (assume___sqr4_rs, assert___sqr4_rs, assume_proof___sqr4_rs,
-           assert_proof___sqr4_rs));
+    trace___sqr4_rs <-
+    (trace___sqr4_rs ++
+    [(Assert,
+     (eqmod
+     (foldr (fun x => (fun (acc:int) => (x + acc))) 0
+     (map (fun ii => ((pow 2 (64 * ii)) * (u64i r.[ii]))) (iota_ 0 4)))
+     ((foldr (fun x => (fun (acc:int) => (x + acc))) 0
+      (map (fun ii => ((pow 2 (64 * ii)) * (u64i old_xa.[ii]))) (iota_ 0 4))) *
+     (foldr (fun x => (fun (acc:int) => (x + acc))) 0
+     (map (fun ii => ((pow 2 (64 * ii)) * (u64i old_xa.[ii]))) (iota_ 0 4))))
+     (single ((pow 2 255) - 19))))]);
+    return (r, trace___sqr4_rs);
   }
 }.
 
-(* All assume are valid. *)
+(* The post is in the trace. *)
 
-lemma __reduce4_assume  : hoare [M.__reduce4 : true ==> (assume_proof_ res)].
-proof.
-    proc. 
-     seq 21 : (assume_proof__ (assume___reduce4, assert___reduce4, assume_proof___reduce4, assert_proof___reduce4)). auto => />.
-     seq 13 : (assume_proof__ (assume___reduce4, assert___reduce4, assume_proof___reduce4, assert_proof___reduce4)). auto => />.
-     seq 16 : (assume_proof__ (assume___reduce4, assert___reduce4, assume_proof___reduce4, assert_proof___reduce4)). auto => />.
-     seq 12 : (assume_proof__ (assume___reduce4, assert___reduce4, assume_proof___reduce4, assert_proof___reduce4)). auto => />. auto => />.
-     seq 7 : (assume_proof__ (assume___reduce4, assert___reduce4, assume_proof___reduce4, assert_proof___reduce4)). auto => />. auto => />.
-     auto => />.
-qed.
-
-lemma __sqr4_rs_assume  : hoare [M.__sqr4_rs : true ==> (assume_proof_ res)].
-proof.
-    proc. wp.
-    call __reduce4_assume.
-    seq 32: ( assume_proof__ (assume___sqr4_rs, assert___sqr4_rs, assume_proof___sqr4_rs, assert_proof___sqr4_rs)). auto => />.
-    seq 15: ( assume_proof__ (assume___sqr4_rs, assert___sqr4_rs, assume_proof___sqr4_rs, assert_proof___sqr4_rs)). auto => />.
-    seq 21: ( assume_proof__ (assume___sqr4_rs, assert___sqr4_rs, assume_proof___sqr4_rs, assert_proof___sqr4_rs)). auto => />.
-    seq 25: ( assume_proof__ (assume___sqr4_rs, assert___sqr4_rs, assume_proof___sqr4_rs, assert_proof___sqr4_rs)). auto => />.
-    seq 38: ( assume_proof__ (assume___sqr4_rs, assert___sqr4_rs, assume_proof___sqr4_rs, assert_proof___sqr4_rs)). auto => />.
-    seq 15: ( assume_proof__ (assume___sqr4_rs, assert___sqr4_rs, assume_proof___sqr4_rs, assert_proof___sqr4_rs)). auto => />. auto => />.
-qed.
-
-(* Soundness of assert/assume. *)
-
-lemma __reduce4_assert_assume_sound  :
-      hoare [M.__reduce4 : true ==> (soundness_ res)].
-proof.
-    proc.
-    seq 20: ( soundness__ (assume___reduce4, assert___reduce4, assume_proof___reduce4, assert_proof___reduce4)). auto => />.
-    seq 18: ( soundness__ (assume___reduce4, assert___reduce4, assume_proof___reduce4, assert_proof___reduce4)). auto => />. smt().
-    seq 12: ( soundness__ (assume___reduce4, assert___reduce4, assume_proof___reduce4, assert_proof___reduce4)). auto => />. smt(). 
-    seq 3: ( soundness__ (assume___reduce4, assert___reduce4, assume_proof___reduce4, assert_proof___reduce4)). auto => />. auto => />.
-    seq 13: ( soundness__ (assume___reduce4, assert___reduce4, assume_proof___reduce4, assert_proof___reduce4)). auto => />. smt().
-    seq 3: ( soundness__ (assume___reduce4, assert___reduce4, assume_proof___reduce4, assert_proof___reduce4)). auto => />. auto => />.
-    auto => />. smt().
-qed.
-
-lemma __sqr4_rs_assert_assume_sound  :
-      hoare [M.__sqr4_rs : true ==> (soundness_ res)].
-proof.
-    proc. wp.
-    call __reduce4_assert_assume_sound.
-    seq 32: ( soundness__ (assume___sqr4_rs, assert___sqr4_rs, assume_proof___sqr4_rs, assert_proof___sqr4_rs)). auto => />.
-    seq 15: ( soundness__ (assume___sqr4_rs, assert___sqr4_rs, assume_proof___sqr4_rs, assert_proof___sqr4_rs)). auto => />. smt().
-    seq 21: ( soundness__ (assume___sqr4_rs, assert___sqr4_rs, assume_proof___sqr4_rs, assert_proof___sqr4_rs)). auto => />. smt().
-    seq 25: ( soundness__ (assume___sqr4_rs, assert___sqr4_rs, assume_proof___sqr4_rs, assert_proof___sqr4_rs)). auto => />. smt().
-    seq 37: ( soundness__ (assume___sqr4_rs, assert___sqr4_rs, assume_proof___sqr4_rs, assert_proof___sqr4_rs)). auto => />. smt().
-    seq 16: ( soundness__ (assume___sqr4_rs, assert___sqr4_rs, assume_proof___sqr4_rs, assert_proof___sqr4_rs)). auto => />. smt().
-    wp. skip. auto => />. smt(). 
-qed.
-(* Lemmas proved by cryptoline. *)
-
-axiom __reduce4_assert _z :
+lemma __reduce4_valid_post _z :
       hoare [M.__reduce4 :
-      ((_z = z) /\ true) ==>
-      (_assert_spec res
+      (_z = z) ==>
+      ((valid (trace res)) =>
       (eqmod
-      (foldr (fun x => (fun (acc: int) => (x + acc))) 0
+      (foldr (fun x => (fun (acc:int) => (x + acc))) 0
       (map (fun ii => ((pow 2 (64 * ii)) * (u64i res.`1.[ii]))) (iota_ 0 4)))
-      (foldr (fun x => (fun (acc: int) => (x + acc))) 0
+      (foldr (fun x => (fun (acc:int) => (x + acc))) 0
       (map (fun ii => ((pow 2 (64 * ii)) * (u64i _z.[ii]))) (iota_ 0 8)))
       (single ((pow 2 255) - 19))))].
+proof.
+proc .
+wp -1 => /=.
+conseq (:  _ ==> (_z = old_z)).
+move => ? _ /> 2?.
+rewrite /trace /= valid_cat /valid //=.
+seq 1 : ((_z = old_z)).
+by auto .
+by conseq  />.
+qed .
 
-axiom __sqr4_rs_assert _xa :
+lemma __sqr4_rs_valid_post _xa :
       hoare [M.__sqr4_rs :
-      ((_xa = xa) /\ true) ==>
-      (_assert_spec res
+      (_xa = xa) ==>
+      ((valid (trace res)) =>
       (eqmod
-      (foldr (fun x => (fun (acc: int) => (x + acc))) 0
+      (foldr (fun x => (fun (acc:int) => (x + acc))) 0
       (map (fun ii => ((pow 2 (64 * ii)) * (u64i res.`1.[ii]))) (iota_ 0 4)))
-      ((foldr (fun x => (fun (acc: int) => (x + acc))) 0
+      ((foldr (fun x => (fun (acc:int) => (x + acc))) 0
        (map (fun ii => ((pow 2 (64 * ii)) * (u64i _xa.[ii]))) (iota_ 0 4))) *
-      (foldr (fun x => (fun (acc: int) => (x + acc))) 0
+      (foldr (fun x => (fun (acc:int) => (x + acc))) 0
       (map (fun ii => ((pow 2 (64 * ii)) * (u64i _xa.[ii]))) (iota_ 0 4))))
       (single ((pow 2 255) - 19))))].
+proof.
+proc .
+wp -1 => /=.
+conseq (:  _ ==> (_xa = old_xa)).
+move => ? _ /> 2?.
+rewrite /trace /= valid_cat /valid //=.
+seq 1 : ((_xa = old_xa)).
+by auto .
+by conseq  />.
+qed .
+
+(* The post is in the trace and all assumes are valid. *)
+
+lemma __reduce4_assume_ _z :
+      hoare [M.__reduce4 :
+      (_z = z) ==> (true => (validk Assume (trace res)))].
+proof.
+    proc. do 2! unroll for ^while. auto => />.
+qed.
+
+lemma __reduce4_assume _z :
+      hoare [M.__reduce4 :
+      (_z = z) ==>
+      (((valid (trace res)) =>
+       (eqmod
+       (foldr (fun x => (fun (acc:int) => (x + acc))) 0
+       (map (fun ii => ((pow 2 (64 * ii)) * (u64i res.`1.[ii]))) (iota_ 0 4))
+       )
+       (foldr (fun x => (fun (acc:int) => (x + acc))) 0
+       (map (fun ii => ((pow 2 (64 * ii)) * (u64i _z.[ii]))) (iota_ 0 8)))
+       (single ((pow 2 255) - 19)))) /\
+      (true => (validk Assume (trace res))))].
+proof.
+conseq (__reduce4_assume_ _z) (__reduce4_valid_post _z) => />.
+qed .
+
+lemma __sqr4_rs_assume_ _xa :
+      hoare [M.__sqr4_rs :
+      (_xa = xa) ==> (true => (validk Assume (trace res)))].
+proof.
+    proc. wp.
+    seq 2: (#pre /\ validk Assume (trace___sqr4_rs)). auto => />.
+    seq 30: (#pre). auto => />. move => &hr H. rewrite !validk_cat //=; 1:smt(@Jcheck @W64 @JUtils).  
+    seq 13: (#pre). auto => />. move => &hr H. rewrite !validk_cat //=; 1:smt(@Jcheck @W64 @JUtils).  
+    seq 19: (#pre). auto => />. move => &hr H. rewrite !validk_cat //=; 1:smt(@Jcheck @W64 @JUtils).  
+    seq 23: (#pre). auto => />. move => &hr H. rewrite !validk_cat //=; 1:smt(@Jcheck @W64 @JUtils).  
+    seq 35: (#pre). auto => />. move => &hr H. rewrite !validk_cat //=; 1:smt(@Jcheck @W64 @JUtils).  
+    seq 10: (#pre). auto => />. move => &hr H. rewrite !validk_cat //=; 1:smt(@Jcheck @W64 @JUtils).  
+    inline M.__reduce4. do 2! unroll for ^while. auto => />.
+    move => &hr H. rewrite !/trace //= !validk_cat //=. move => H0 H1.
+    rewrite !H1 !b2i0 => />. rewrite !valid_cat //=. smt(forall_validk_valid).
+qed.
+
+lemma __sqr4_rs_assume _xa :
+      hoare [M.__sqr4_rs :
+      (_xa = xa) ==>
+      (((valid (trace res)) =>
+       (eqmod
+       (foldr (fun x => (fun (acc:int) => (x + acc))) 0
+       (map (fun ii => ((pow 2 (64 * ii)) * (u64i res.`1.[ii]))) (iota_ 0 4))
+       )
+       ((foldr (fun x => (fun (acc:int) => (x + acc))) 0
+        (map (fun ii => ((pow 2 (64 * ii)) * (u64i _xa.[ii]))) (iota_ 0 4))) *
+       (foldr (fun x => (fun (acc:int) => (x + acc))) 0
+       (map (fun ii => ((pow 2 (64 * ii)) * (u64i _xa.[ii]))) (iota_ 0 4))))
+       (single ((pow 2 255) - 19)))) /\
+      (true => (validk Assume (trace res))))].
+proof.
+conseq (__sqr4_rs_assume_ _xa) (__sqr4_rs_valid_post _xa) => />.
+qed .
+
+(* All assert are valid. *)
+
+lemma __reduce4_assert _z :
+      hoare [M.__reduce4 :
+      ((_z = z) /\ true) ==> (validk Assert (trace res))].
+proof.
+admitted (* Proven by Cryptoline *).
+
+lemma __sqr4_rs_assert _xa :
+      hoare [M.__sqr4_rs :
+      ((_xa = xa) /\ true) ==> (validk Assert (trace res))].
+proof.
+admitted (* Proven by Cryptoline *).
 
 (* Final specification for the functions. *)
 
-lemma __reduce4_spec  :
-      forall _z,
+lemma __reduce4_spec _z :
       hoare [M.__reduce4 :
       ((_z = z) /\ true) ==>
       (eqmod
-      (foldr (fun x => (fun (acc: int) => (x + acc))) 0
+      (foldr (fun x => (fun (acc:int) => (x + acc))) 0
       (map (fun ii => ((pow 2 (64 * ii)) * (u64i res.`1.[ii]))) (iota_ 0 4)))
-      (foldr (fun x => (fun (acc: int) => (x + acc))) 0
+      (foldr (fun x => (fun (acc:int) => (x + acc))) 0
       (map (fun ii => ((pow 2 (64 * ii)) * (u64i _z.[ii]))) (iota_ 0 8)))
       (single ((pow 2 255) - 19)))].
 proof.
-move => _z.
-have h  :
-     hoare [M.__reduce4 :
-     ((_z = z) /\ true) ==>
-     (_spec_soundness res
-     (eqmod
-     (foldr (fun x => (fun (acc: int) => (x + acc))) 0
-     (map (fun ii => ((pow 2 (64 * ii)) * (u64i res.`1.[ii]))) (iota_ 0 4)))
-     (foldr (fun x => (fun (acc: int) => (x + acc))) 0
-     (map (fun ii => ((pow 2 (64 * ii)) * (u64i _z.[ii]))) (iota_ 0 8)))
-     (single ((pow 2 255) - 19))))].
-by conseq __reduce4_assume (__reduce4_assert _z).
-conseq h __reduce4_assert_assume_sound => // ; smt ().
+conseq (__reduce4_assume _z) (__reduce4_assert _z) => />.
+smt (all_validk_valid).
 qed .
 
-lemma __sqr4_rs_spec  :
-      forall _xa,
+lemma __sqr4_rs_spec _xa :
       hoare [M.__sqr4_rs :
       ((_xa = xa) /\ true) ==>
       (eqmod
-      (foldr (fun x => (fun (acc: int) => (x + acc))) 0
+      (foldr (fun x => (fun (acc:int) => (x + acc))) 0
       (map (fun ii => ((pow 2 (64 * ii)) * (u64i res.`1.[ii]))) (iota_ 0 4)))
-      ((foldr (fun x => (fun (acc: int) => (x + acc))) 0
+      ((foldr (fun x => (fun (acc:int) => (x + acc))) 0
        (map (fun ii => ((pow 2 (64 * ii)) * (u64i _xa.[ii]))) (iota_ 0 4))) *
-      (foldr (fun x => (fun (acc: int) => (x + acc))) 0
+      (foldr (fun x => (fun (acc:int) => (x + acc))) 0
       (map (fun ii => ((pow 2 (64 * ii)) * (u64i _xa.[ii]))) (iota_ 0 4))))
       (single ((pow 2 255) - 19)))].
 proof.
-move => _xa.
-have h  :
-     hoare [M.__sqr4_rs :
-     ((_xa = xa) /\ true) ==>
-     (_spec_soundness res
-     (eqmod
-     (foldr (fun x => (fun (acc: int) => (x + acc))) 0
-     (map (fun ii => ((pow 2 (64 * ii)) * (u64i res.`1.[ii]))) (iota_ 0 4)))
-     ((foldr (fun x => (fun (acc: int) => (x + acc))) 0
-      (map (fun ii => ((pow 2 (64 * ii)) * (u64i _xa.[ii]))) (iota_ 0 4))) *
-     (foldr (fun x => (fun (acc: int) => (x + acc))) 0
-     (map (fun ii => ((pow 2 (64 * ii)) * (u64i _xa.[ii]))) (iota_ 0 4))))
-     (single ((pow 2 255) - 19))))].
-by conseq __sqr4_rs_assume (__sqr4_rs_assert _xa).
-conseq h __sqr4_rs_assert_assume_sound => // ; smt ().
+conseq (__sqr4_rs_assume _xa) (__sqr4_rs_assert _xa) => />.
+smt (all_validk_valid).
 qed .
-
