proof/crypto_scalarmult/curve25519/amd64/cryptoline_extraction/Sub4Extracted.ec
@@ -1,25 +1,24 @@
-require import AllCore Int IntDiv CoreMap List Distr.
+require import AllCore IntDiv CoreMap List Distr.
 
 from Jasmin require import JModel_x86.
 
-require import Jcheck Zp_limbs Zp_25519 CommonCryptoline.
-import Zp_25519 Zp Zp_limbs EClib.
-
-
 import SLH64.
 
-require import Jcheck.
+from Jasmin require import Jcheck.
 
 require import Array4.
 
 require import WArray32.
 
+require import Zp_limbs Zp_25519 CommonCryptoline.
+import Zp_25519 Zp Zp_limbs EClib.
+
 module M = {
-  var tmp__check : to_check
+  var tmp__trace : trace
   var tmp__data___sub4_rrs : (W64.t Array4.t)
   var tmp____sub4_rrs : W64.t Array4.t
   proc __sub4_rrs (f:W64.t Array4.t, gs:W64.t Array4.t) : ((W64.t Array4.t) *
-                                                          to_check) = {
+                                                          trace) = {
     var aux:bool;
     var aux_1:int;
     var aux_0:W64.t;
@@ -33,14 +32,12 @@ module M = {
     var  _2:bool;
     var  _3:bool;
     var  _4:bool;
-    var assume___sub4_rrs:bool;
-    var assert___sub4_rrs:bool;
-    var assume_proof___sub4_rrs:bool;
-    var assert_proof___sub4_rrs:bool;
-    assume___sub4_rrs <- true;
-    assert___sub4_rrs <- true;
-    assume_proof___sub4_rrs <- true;
-    assert_proof___sub4_rrs <- assert___sub4_rrs;
+    var old_gs:W64.t Array4.t;
+    var old_f:W64.t Array4.t;
+    var trace___sub4_rrs:trace;
+    old_f <- f;
+    old_gs <- gs;
+    trace___sub4_rrs <- [];
     h <- witness;
     ( _0,  _1,  _2,  _3,  _4, z) <- (set0_64);
     h <- (copy_64 f);
@@ -56,27 +53,16 @@ module M = {
     }
     borrowo <- cf;
     (cf, z) <- (sbb_64 z z cf);
-    assert_proof___sub4_rrs <-
-    (assert_proof___sub4_rrs /\
-    ((assert___sub4_rrs /\ assume___sub4_rrs) => (cf = borrowo)));
-    assert___sub4_rrs <- (assert___sub4_rrs /\ (cf = borrowo));
-    assume_proof___sub4_rrs <-
-    (assume_proof___sub4_rrs /\
-    ((assert___sub4_rrs /\ assume___sub4_rrs) => ((b2i cf) = (b2i borrowo))));
-    assume___sub4_rrs <- (assume___sub4_rrs /\ ((b2i cf) = (b2i borrowo)));
+    trace___sub4_rrs <- (trace___sub4_rrs ++ [(Assert, (cf = borrowo))]);
+    trace___sub4_rrs <-
+    (trace___sub4_rrs ++ [(Assume, ((b2i cf) = (b2i borrowo)))]);
     z <- (z `&` (W64.of_int 38));
-    assert_proof___sub4_rrs <-
-    (assert_proof___sub4_rrs /\
-    ((assert___sub4_rrs /\ assume___sub4_rrs) =>
-    (((! cf) /\ (z = (W64.of_int 0))) \/ (cf /\ (z = (W64.of_int 38))))));
-    assert___sub4_rrs <-
-    (assert___sub4_rrs /\
-    (((! cf) /\ (z = (W64.of_int 0))) \/ (cf /\ (z = (W64.of_int 38)))));
-    assume_proof___sub4_rrs <-
-    (assume_proof___sub4_rrs /\
-    ((assert___sub4_rrs /\ assume___sub4_rrs) =>
-    ((u64i z) = ((b2i cf) * 38))));
-    assume___sub4_rrs <- (assume___sub4_rrs /\ ((u64i z) = ((b2i cf) * 38)));
+    trace___sub4_rrs <-
+    (trace___sub4_rrs ++
+    [(Assert,
+     (((! cf) /\ (z = (W64.of_int 0))) \/ (cf /\ (z = (W64.of_int 38)))))]);
+    trace___sub4_rrs <-
+    (trace___sub4_rrs ++ [(Assume, ((u64i z) = ((b2i cf) * 38)))]);
     (aux, aux_0) <- (sbb_64 h.[0] z false);
     cf <- aux;
     h.[0] <- aux_0;
@@ -89,107 +75,117 @@ module M = {
     }
     borrowo <- cf;
     (cf, z) <- (sbb_64 z z cf);
-    assert_proof___sub4_rrs <-
-    (assert_proof___sub4_rrs /\
-    ((assert___sub4_rrs /\ assume___sub4_rrs) => (cf = borrowo)));
-    assert___sub4_rrs <- (assert___sub4_rrs /\ (cf = borrowo));
-    assume_proof___sub4_rrs <-
-    (assume_proof___sub4_rrs /\
-    ((assert___sub4_rrs /\ assume___sub4_rrs) => ((b2i cf) = (b2i borrowo))));
-    assume___sub4_rrs <- (assume___sub4_rrs /\ ((b2i cf) = (b2i borrowo)));
+    trace___sub4_rrs <- (trace___sub4_rrs ++ [(Assert, (cf = borrowo))]);
+    trace___sub4_rrs <-
+    (trace___sub4_rrs ++ [(Assume, ((b2i cf) = (b2i borrowo)))]);
     z <- (z `&` (W64.of_int 38));
-    assert_proof___sub4_rrs <-
-    (assert_proof___sub4_rrs /\
-    ((assert___sub4_rrs /\ assume___sub4_rrs) =>
-    (((! cf) /\ (z = (W64.of_int 0))) \/ (cf /\ (z = (W64.of_int 38))))));
-    assert___sub4_rrs <-
-    (assert___sub4_rrs /\
-    (((! cf) /\ (z = (W64.of_int 0))) \/ (cf /\ (z = (W64.of_int 38)))));
-    assume_proof___sub4_rrs <-
-    (assume_proof___sub4_rrs /\
-    ((assert___sub4_rrs /\ assume___sub4_rrs) =>
-    ((u64i z) = ((b2i cf) * 38))));
-    assume___sub4_rrs <- (assume___sub4_rrs /\ ((u64i z) = ((b2i cf) * 38)));
+    trace___sub4_rrs <-
+    (trace___sub4_rrs ++
+    [(Assert,
+     (((! cf) /\ (z = (W64.of_int 0))) \/ (cf /\ (z = (W64.of_int 38)))))]);
+    trace___sub4_rrs <-
+    (trace___sub4_rrs ++ [(Assume, ((u64i z) = ((b2i cf) * 38)))]);
     (aux, aux_0) <- (sbb_64 h.[0] z false);
     cf <- aux;
     h.[0] <- aux_0;
-    assert_proof___sub4_rrs <-
-    (assert_proof___sub4_rrs /\
-    ((assert___sub4_rrs /\ assume___sub4_rrs) => (! cf)));
-    assert___sub4_rrs <- (assert___sub4_rrs /\ (! cf));
-    assume_proof___sub4_rrs <-
-    (assume_proof___sub4_rrs /\
-    ((assert___sub4_rrs /\ assume___sub4_rrs) => ((b2i cf) = 0)));
-    assume___sub4_rrs <- (assume___sub4_rrs /\ ((b2i cf) = 0));
-    return (h, (assume___sub4_rrs, assert___sub4_rrs, assume_proof___sub4_rrs, assert_proof___sub4_rrs));
+    trace___sub4_rrs <- (trace___sub4_rrs ++ [(Assert, (! cf))]);
+    trace___sub4_rrs <- (trace___sub4_rrs ++ [(Assume, ((b2i cf) = 0))]);
+    trace___sub4_rrs <-
+    (trace___sub4_rrs ++
+    [(Assert,
+     (eqmod
+     (foldr (fun x => (fun (acc:int) => (x + acc))) 0
+     (map (fun ii => ((pow 2 (64 * ii)) * (u64i h.[ii]))) (iota_ 0 4)))
+     ((foldr (fun x => (fun (acc:int) => (x + acc))) 0
+      (map (fun ii => ((pow 2 (64 * ii)) * (u64i old_f.[ii]))) (iota_ 0 4))) -
+     (foldr (fun x => (fun (acc:int) => (x + acc))) 0
+     (map (fun ii => ((pow 2 (64 * ii)) * (u64i old_gs.[ii]))) (iota_ 0 4))))
+     (single ((pow 2 255) - 19))))]);
+    return (h, trace___sub4_rrs);
   }
 }.
 
+(* The post is in the trace. *)
 
-(* All assume are valid. *)
-
-lemma __sub4_rrs_assume  :
-      hoare [M.__sub4_rrs : true ==> (assume_proof_ res)].
+lemma __sub4_rrs_valid_post _f _gs :
+      hoare [M.__sub4_rrs :
+      ((_gs = gs) /\ (_f = f)) ==>
+      ((valid (trace res)) =>
+      (eqmod
+      (foldr (fun x => (fun (acc:int) => (x + acc))) 0
+      (map (fun ii => ((pow 2 (64 * ii)) * (u64i res.`1.[ii]))) (iota_ 0 4)))
+      ((foldr (fun x => (fun (acc:int) => (x + acc))) 0
+       (map (fun ii => ((pow 2 (64 * ii)) * (u64i _f.[ii]))) (iota_ 0 4))) -
+      (foldr (fun x => (fun (acc:int) => (x + acc))) 0
+      (map (fun ii => ((pow 2 (64 * ii)) * (u64i _gs.[ii]))) (iota_ 0 4))))
+      (single ((pow 2 255) - 19))))].
 proof.
-    proc. do 2! unroll for ^while.
-    wp; skip => />. move => &hr.
+proc .
+wp -1 => /=.
+conseq (:  _ ==> ((_gs = old_gs) /\ (_f = old_f))).
+move => ? _ /> 2?.
+rewrite /trace /= valid_cat /valid //=.
+seq 4 : (((_gs = old_gs) /\ (_f = old_f))).
+by auto . 
+do 2! unroll for ^while.
+by conseq  />.
+qed .
+
+(* The post is in the trace and all assumes are valid. *)
+
+lemma __sub4_rrs_assume_ _f _gs :
+      hoare [M.__sub4_rrs :
+      ((_gs = gs) /\ (_f = f)) ==> (true => (validk Assume (trace res)))].
+proof.
+    proc. 
+    wp -1 => /=. do 2! unroll for ^while. wp; skip => />. move => H. 
+    do split. by rewrite H. move => H1. 
+    do split. rewrite H. smt(@W64 @JUtils). move => H2. 
+    do split. rewrite H2. smt(@W64 @JUtils). move => H3.
     smt(@W64 @JUtils).
 qed.
 
-(* Soundness of assert/assume. *)
-
-lemma __sub4_rrs_assert_assume_sound  :
-      hoare [M.__sub4_rrs : true ==> (soundness_ res)].
-proof.
-    proc. do 2! unroll for ^while.
-    wp; skip => />. move => &hr.
-    smt(@W64 @JUtils). 
-qed.
-
-(* Lemmas proved by cryptoline. *)
-
-axiom __sub4_rrs_assert _f _gs :
+lemma __sub4_rrs_assume _f _gs :
       hoare [M.__sub4_rrs :
-      (((_gs = gs) /\ (_f = f)) /\ true) ==>
-      (_assert_spec res
-      (eqmod
-      (foldr (fun x => (fun (acc: int) => (x + acc))) 0
-      (map (fun ii => ((pow 2 (64 * ii)) * (u64i res.`1.[ii]))) (iota_ 0 4)))
-      ((foldr (fun x => (fun (acc: int) => (x + acc))) 0
-       (map (fun ii => ((pow 2 (64 * ii)) * (u64i _f.[ii]))) (iota_ 0 4))) -
-      (foldr (fun x => (fun (acc: int) => (x + acc))) 0
-      (map (fun ii => ((pow 2 (64 * ii)) * (u64i _gs.[ii]))) (iota_ 0 4))))
-      (single ((pow 2 255) - 19))))].
+      ((_gs = gs) /\ (_f = f)) ==>
+      (((valid (trace res)) =>
+       (eqmod
+       (foldr (fun x => (fun (acc:int) => (x + acc))) 0
+       (map (fun ii => ((pow 2 (64 * ii)) * (u64i res.`1.[ii]))) (iota_ 0 4))
+       )
+       ((foldr (fun x => (fun (acc:int) => (x + acc))) 0
+        (map (fun ii => ((pow 2 (64 * ii)) * (u64i _f.[ii]))) (iota_ 0 4))) -
+       (foldr (fun x => (fun (acc:int) => (x + acc))) 0
+       (map (fun ii => ((pow 2 (64 * ii)) * (u64i _gs.[ii]))) (iota_ 0 4))))
+       (single ((pow 2 255) - 19)))) /\
+      (true => (validk Assume (trace res))))].
+proof.
+conseq (__sub4_rrs_assume_ _f _gs) (__sub4_rrs_valid_post _f _gs) => />.
+qed .
+
+(* All assert are valid. *)
+
+lemma __sub4_rrs_assert _f _gs :
+      hoare [M.__sub4_rrs :
+      (((_gs = gs) /\ (_f = f)) /\ true) ==> (validk Assert (trace res))].
+proof.
+admitted (* Proven by Cryptoline *).
 
 (* Final specification for the functions. *)
 
-lemma __sub4_rrs_spec  :
-      forall _f _gs,
+lemma __sub4_rrs_spec _f _gs :
       hoare [M.__sub4_rrs :
       (((_gs = gs) /\ (_f = f)) /\ true) ==>
       (eqmod
-      (foldr (fun x => (fun (acc: int) => (x + acc))) 0
+      (foldr (fun x => (fun (acc:int) => (x + acc))) 0
       (map (fun ii => ((pow 2 (64 * ii)) * (u64i res.`1.[ii]))) (iota_ 0 4)))
-      ((foldr (fun x => (fun (acc: int) => (x + acc))) 0
+      ((foldr (fun x => (fun (acc:int) => (x + acc))) 0
        (map (fun ii => ((pow 2 (64 * ii)) * (u64i _f.[ii]))) (iota_ 0 4))) -
-      (foldr (fun x => (fun (acc: int) => (x + acc))) 0
+      (foldr (fun x => (fun (acc:int) => (x + acc))) 0
       (map (fun ii => ((pow 2 (64 * ii)) * (u64i _gs.[ii]))) (iota_ 0 4))))
       (single ((pow 2 255) - 19)))].
 proof.
-move => _f _gs.
-have h  :
-     hoare [M.__sub4_rrs :
-     (((_gs = gs) /\ (_f = f)) /\ true) ==>
-     (_spec_soundness res
-     (eqmod
-     (foldr (fun x => (fun (acc: int) => (x + acc))) 0
-     (map (fun ii => ((pow 2 (64 * ii)) * (u64i res.`1.[ii]))) (iota_ 0 4)))
-     ((foldr (fun x => (fun (acc: int) => (x + acc))) 0
-      (map (fun ii => ((pow 2 (64 * ii)) * (u64i _f.[ii]))) (iota_ 0 4))) -
-     (foldr (fun x => (fun (acc: int) => (x + acc))) 0
-     (map (fun ii => ((pow 2 (64 * ii)) * (u64i _gs.[ii]))) (iota_ 0 4))))
-     (single ((pow 2 255) - 19))))].
-by conseq __sub4_rrs_assume (__sub4_rrs_assert _f _gs).
-conseq h __sub4_rrs_assert_assume_sound => // ; smt ().
+conseq (__sub4_rrs_assume _f _gs) (__sub4_rrs_assert _f _gs) => />.
+smt (all_validk_valid).
 qed .
 
