proof/crypto_scalarmult/curve25519/amd64/ref4/CryptolineEquivs_Ref4.ec
@@ -1,85 +1,103 @@
-require import Int Ref4_scalarmult_s Jcheck Add4Extracted Sub4Extracted Mul4RefExtracted Mul4_a24RefExtracted Int Sqr4RefExtracted.
+require import Int Ref4_scalarmult_s Add4Extracted Sub4Extracted Mul4RefExtracted Mul4_a24RefExtracted Int Sqr4RefExtracted CommonToBytes_0p CommonToBytes_p2_255 CommonToBytes_2p2_256 CommonToBytes_2_2552p.
 
-from Jasmin require import JWord.
+from Jasmin require import JWord Jcheck.
 
-require import Array8.
+require import Array4 Array8.
 
 lemma __add4_rrs_cryptoline_equiv_ref4  :
       equiv [Ref4_scalarmult_s.M.__add4_rrs ~ Add4Extracted.M.__add4_rrs : ={f, g} ==> res{1} = res{2}.`1].
 proof.
     proc. 
-    seq 9 14 : (={f, g, h, z} /\  _1{1} = cf{2}). by sim.
-    seq 7 20 : (={f, g, h, z} /\ _2{1} = cf{2}). by sim.
-    sim : (={f, g, h, z}). auto => />. 
-    rewrite addcE /carry_add b2i0 => />. 
+    unroll for{1} ^while.
+    unroll for{1} ^while.
+    unroll for{2} ^while.
+    unroll for{2} ^while. auto => />.
+    move => *. rewrite !/copy_64 !/set0_64_ => />. 
+    apply Array4.ext_eq. move => i ib. rewrite !get_setE 1..18://=.
+    case (i = 0) => I0. smt(@W64).
+    case (i = 1) => I1. smt(@W64).
+    case (i = 2) => I2. smt(@W64).
+    case (i = 3) => I3. smt(@W64). smt().      
 qed.
 
 lemma __sub4_rss_cryptoline_equiv_ref4  :
       equiv [Ref4_scalarmult_s.M.__sub4_rrs ~ Sub4Extracted.M.__sub4_rrs : ={f, gs} ==> res{1} = res{2}.`1].
 proof.
-    proc.  
-    seq 9 14 : (={f, gs, h, z} /\  _1{1} = cf{2}). by sim.
-    seq 7 16 : (={f, gs, h, z} /\ _2{1} = cf{2}). by sim.
-    sim : (={f, gs, h, z}). auto => />.
-    rewrite subcE /borrow_sub b2i0 => />. 
+    proc.     
+    unroll for{1} ^while.
+    unroll for{1} ^while.
+    unroll for{2} ^while.
+    unroll for{2} ^while. auto => />.
+    move => *. rewrite !/copy_64 !/set0_64_ => />. 
+    apply Array4.ext_eq. move => i ib. rewrite !get_setE 1..18://=.
+    case (i = 0) => I0. smt(@W64).
+    case (i = 1) => I1. smt(@W64).
+    case (i = 2) => I2. smt(@W64).
+    case (i = 3) => I3. smt(@W64). smt().  
 qed.
 
 lemma __reduce_cryptoline_equiv_ref4  :
       equiv [Ref4_scalarmult_s.M.__reduce4 ~ Mul4RefExtracted.M.__reduce4 : ={z} ==> res{1} = res{2}.`1].
 proof.
-    proc.
-    seq 36 52 : (={r, r38, rax, h, l, i, z, z8, cf}). by sim. 
-    seq 6 14 : (={r, r38, rax, h, l, i, z, z8, r0, cf}). auto => />.
-    rewrite !addcE !/carry_add !muluE !/mulhi => />. 
-    seq 2 2 : (={r, r38, rax, h, l, i, z8, z, r0, cf}). by sim.
-    sim : (={r, r38, rax, h, l, i, z8, r0, z}). auto => />.
-    move => *. do split. 
-    rewrite !/mulhi !/mulu !addcE !/carry_add => />. 
-    rewrite !/mulhi !/mulu !addcE !/carry_add => />. 
+    proc.     
+    unroll for{1} ^while.
+    unroll for{1} ^while.
+    unroll for{2} ^while.
+    unroll for{2} ^while. auto => />.
+    move => *. rewrite !/copy_64 !/set0_64_ => />. 
+    apply Array4.ext_eq. move => i ib. rewrite !get_setE 1..26://=.
+    case (i = 0) => I0. smt(@W64).
+    case (i = 1) => I1. smt(@W64).
+    case (i = 2) => I2. smt(@W64).
+    case (i = 3) => I3. smt(@W64). smt().    
 qed.
 
 lemma __reduce_cryptoline_equiv_sqr_ref4  :
       equiv [Ref4_scalarmult_s.M.__reduce4 ~ Sqr4RefExtracted.M.__reduce4 : ={z} ==> res{1} = res{2}.`1].
 proof.
-    proc.
-    seq 36 52 : (={r, r38, rax, h, l, i, z, z8, cf}). by sim. 
-    seq 6 14 : (={r, r38, rax, h, l, i, z, z8, r0, cf}). auto => />.
-    rewrite !addcE !/carry_add !muluE !/mulhi => />. 
-    seq 2 2 : (={r, r38, rax, h, l, i, z8, z, r0, cf}). by sim.
-    sim : (={r, r38, rax, h, l, i, z8, r0, z}). auto => />.
-    move => *. do split. 
-    rewrite !/mulhi !/mulu !addcE !/carry_add => />. 
-    rewrite !/mulhi !/mulu !addcE !/carry_add => />. 
+    proc.     
+    unroll for{1} ^while.
+    unroll for{1} ^while.
+    unroll for{2} ^while.
+    unroll for{2} ^while. auto => />.
+    move => *. rewrite !/copy_64 !/set0_64_ => />. 
+    apply Array4.ext_eq. move => i ib. rewrite !get_setE 1..26://=.
+    case (i = 0) => I0. smt(@W64).
+    case (i = 1) => I1. smt(@W64).
+    case (i = 2) => I2. smt(@W64).
+    case (i = 3) => I3. smt(@W64). smt(). 
 qed.
-
 
 lemma __mul4_rss_cryptoline_equiv_ref4  :
       equiv [Ref4_scalarmult_s.M.__mul4_rss ~ Mul4RefExtracted.M.__mul4_rss : ={xa, ya} ==> res{1} = res{2}.`1].
 proof.
-    proc.     
-    wp. call __reduce_cryptoline_equiv_ref4.
-    seq 9 13 : (={x, y, z, r, xa, ya}). by sim.
-    unroll for{1} ^while. unroll for{2} ^while.
-    seq 4 4 : (={x, y, z, r, xa, ya, hprev, i}).  
-    unroll for{1} ^while. unroll for{2} ^while.
-    rcondt{1} ^if. auto => />. rcondt{2} ^if. auto => />. sim.
-    seq 4 4 : (={x, y, z, r, xa, ya, hprev, i}).  
-    unroll for{1} ^while. unroll for{2} ^while.
-    rcondt{1} ^if. auto => />. rcondt{2} ^if. auto => />. sim.
-    seq 4 4 : (={x, y, z, r, xa, ya, hprev, i}).  
-    unroll for{1} ^while. unroll for{2} ^while.
-    rcondt{1} ^if. auto => />. rcondt{2} ^if. auto => />. sim.
-    wp. skip. auto => />.
+    proc. wp.       
+    unroll for{1} ^while.     
+    unroll for{1} ^while.
+    unroll for{2} ^while.
+    unroll for{2} ^while. 
+    unroll for{2} ^while. 
+    unroll for{2} ^while. 
+    unroll for{2} ^while. 
+    unroll for{2} ^while. 
+    unroll for{1} ^while. 
+    unroll for{1} ^while. 
+    unroll for{1} ^while. 
+    unroll for{1} ^while.
+    call __reduce_cryptoline_equiv_ref4.
+    simplify. sim.      
 qed.
 
 lemma __mul4_a24_rs_cryptoline_equiv_ref4  :
       equiv [Ref4_scalarmult_s.M.__mul4_a24_rs ~ Mul4_a24RefExtracted.M.__mul4_a24_rs : ={xa} /\ a24{1} = W64.of_int 121665 ==> res{1} = res{2}.`1].
 proof.
-    proc. 
-    seq 4 12 : (={r, c, rax, rdx, xa}). auto => />.
-    seq 39 47 : (={r, c, rax, rdx, xa, t1, t2, t3, t4, cf}). auto => />.
-    sim : (={r, c, rax, rdx, xa, t1, t2, t3, t4}). auto => />.
-    move => &2. rewrite !addcE !/carry_add !b2i0  => />.  
+    proc. auto => />.
+    move => *. rewrite !/copy_64 !/set0_64_ => />. 
+    apply Array4.ext_eq. move => i ib. rewrite !get_setE 1..24://=.
+    case (i = 0) => I0. smt(@W64).
+    case (i = 1) => I1. smt(@W64).
+    case (i = 2) => I2. smt(@W64).
+    case (i = 3) => I3. smt(@W64). smt().  
 qed.
 
 lemma __sqr4_rs_cryptoline_equiv_ref4  :
@@ -90,4 +108,27 @@ proof.
     sim : (={zero, xa, r, t, z, rax, rdx, aux, aux_0}). 
 qed.
 
+lemma __tobytes_cryptoline_equiv_0p_ref4  :
+      equiv [Ref4_scalarmult_s.M.__tobytes4 ~ CommonToBytes_0p.M.__tobytes4 : ={f} ==> res{1} = res{2}.`1].
+proof.
+    proc. auto => />.    
+qed.
+
+lemma __tobytes_cryptoline_equiv_p2_255_ref4  :
+      equiv [Ref4_scalarmult_s.M.__tobytes4 ~ CommonToBytes_p2_255.M.__tobytes4 : ={f} ==> res{1} = res{2}.`1].
+proof.
+    proc. auto => />.    
+qed.
+
+lemma __tobytes_cryptoline_equiv_2p2_256_ref4  :
+      equiv [Ref4_scalarmult_s.M.__tobytes4 ~ CommonToBytes_2p2_256.M.__tobytes4 : ={f} ==> res{1} = res{2}.`1].
+proof.
+    proc. auto => />.    
+qed.
+
+lemma __tobytes_cryptoline_equiv_2_2552p_ref4  :
+      equiv [Ref4_scalarmult_s.M.__tobytes4 ~ CommonToBytes_2_2552p.M.__tobytes4 : ={f} ==> res{1} = res{2}.`1].
+proof.
+    proc. auto => />.    
+qed.
 
